ems/SimGlobal.v
@@ -15,18 +15,13 @@ Require Import SimSTS.
 Set Implicit Arguments.
 
 
-
-
-
-
-
 Section SIM.
 
 Section TY.
 (* Context `{R: Type}. *)
 Inductive _simg
-          (simg: forall R0 R1 (RR: R0 -> R1 -> Prop), bool -> bool -> (itree eventE R0) -> (itree eventE R1) -> Prop)
-          {R0 R1} (RR: R0 -> R1 -> Prop) (f_src f_tgt: bool): (itree eventE R0) -> (itree eventE R1) -> Prop :=
+          (simg: forall R0 R1 (RR: R0 -> R1 -> Prop), flag -> flag -> (itree eventE R0) -> (itree eventE R1) -> Prop)
+          {R0 R1} (RR: R0 -> R1 -> Prop) (f_src f_tgt: flag): (itree eventE R0) -> (itree eventE R1) -> Prop :=
 | simg_ret
     r_src r_tgt
     (SIM: RR r_src r_tgt)
@@ -34,61 +29,61 @@ Inductive _simg
     _simg simg RR f_src f_tgt (Ret r_src) (Ret r_tgt)
 | simg_syscall
     ktr_src0 ktr_tgt0 fn varg rvs
-    (SIM: forall x_src x_tgt (EQ: x_src = x_tgt), simg _ _ RR true true (ktr_src0 x_src) (ktr_tgt0 x_tgt))
+    (SIM: forall x_src x_tgt (EQ: x_src = x_tgt), simg _ _ RR TT TT (ktr_src0 x_src) (ktr_tgt0 x_tgt))
   :
     _simg simg RR f_src f_tgt (trigger (Syscall fn varg rvs) >>= ktr_src0) (trigger (Syscall fn varg rvs) >>= ktr_tgt0)
 
 | simg_tauL
     itr_src0 itr_tgt0
     (TAUL: True)
-    (SIM: @_simg simg _ _ RR true f_tgt itr_src0 itr_tgt0)
+    (SIM: @_simg simg _ _ RR TT f_tgt itr_src0 itr_tgt0)
   :
     _simg simg RR f_src f_tgt (tau;; itr_src0) (itr_tgt0)
 | simg_tauR
     itr_src0 itr_tgt0
     (TAUR: True)
-    (SIM: @_simg simg _ _ RR f_src true itr_src0 itr_tgt0)
+    (SIM: @_simg simg _ _ RR f_src TT itr_src0 itr_tgt0)
   :
     _simg simg RR f_src f_tgt (itr_src0) (tau;; itr_tgt0)
 
 | simg_chooseL
     X ktr_src0 itr_tgt0
     (CHOOSEL: True)
-    (SIM: exists x, _simg simg RR true f_tgt (ktr_src0 x) itr_tgt0)
+    (SIM: exists x, _simg simg RR TT f_tgt (ktr_src0 x) itr_tgt0)
   :
     _simg simg RR f_src f_tgt (trigger (Choose X) >>= ktr_src0) (itr_tgt0)
 | simg_chooseR
     X itr_src0 ktr_tgt0
     (CHOOSER: True)
-    (SIM: forall x, _simg simg RR f_src true itr_src0 (ktr_tgt0 x))
+    (SIM: forall x, _simg simg RR f_src TT itr_src0 (ktr_tgt0 x))
   :
     _simg simg RR f_src f_tgt (itr_src0) (trigger (Choose X) >>= ktr_tgt0)
 
 | simg_takeL
     X ktr_src0 itr_tgt0
     (TAKEL: True)
-    (SIM: forall x, _simg simg RR true f_tgt (ktr_src0 x) itr_tgt0)
+    (SIM: forall x, _simg simg RR TT f_tgt (ktr_src0 x) itr_tgt0)
   :
     _simg simg RR f_src f_tgt (trigger (Take X) >>= ktr_src0) (itr_tgt0)
 | simg_takeR
     X itr_src0 ktr_tgt0
     (TAKER: True)
-    (SIM: exists x, _simg simg RR f_src true itr_src0 (ktr_tgt0 x))
+    (SIM: exists x, _simg simg RR f_src TT itr_src0 (ktr_tgt0 x))
   :
     _simg simg RR f_src f_tgt (itr_src0) (trigger (Take X) >>= ktr_tgt0)
 
 | simg_progress
     itr_src itr_tgt
-    (SIM: simg _ _ RR false false itr_src itr_tgt)
-    (SRC: f_src = true)
-    (TGT: f_tgt = true)
+    (SIM: simg _ _ RR BB BB itr_src itr_tgt)
+    (SRC: f_src = TT)
+    (TGT: f_tgt = TT)
   :
     _simg simg RR f_src f_tgt itr_src itr_tgt
 .
 
-Lemma _simg_ind2 (r: forall R0 R1 (RR: R0 -> R1 -> Prop), bool -> bool -> (itree eventE R0) -> (itree eventE R1) -> Prop)
+Lemma _simg_ind2 (r: forall R0 R1 (RR: R0 -> R1 -> Prop), flag -> flag -> (itree eventE R0) -> (itree eventE R1) -> Prop)
       R0 R1 (RR: R0 -> R1 -> Prop)
-      (P: bool -> bool -> (itree eventE R0) -> (itree eventE R1) -> Prop)
+      (P: flag -> flag -> (itree eventE R0) -> (itree eventE R1) -> Prop)
       (RET: forall
           f_src f_tgt
           r_src r_tgt
@@ -97,52 +92,52 @@ Lemma _simg_ind2 (r: forall R0 R1 (RR: R0 -> R1 -> Prop), bool -> bool -> (itree
       (SYSCALL: forall
           f_src f_tgt
           ktr_src0 ktr_tgt0 fn varg rvs
-          (SIM: forall x_src x_tgt (EQ: x_src = x_tgt), r _ _ RR true true (ktr_src0 x_src) (ktr_tgt0 x_tgt)),
+          (SIM: forall x_src x_tgt (EQ: x_src = x_tgt), r _ _ RR TT TT (ktr_src0 x_src) (ktr_tgt0 x_tgt)),
           P f_src f_tgt (trigger (Syscall fn varg rvs) >>= ktr_src0) (trigger (Syscall fn varg rvs) >>= ktr_tgt0))
       (TAUL: forall
           f_src f_tgt
           itr_src0 itr_tgt0
           (TAUL: True)
-          (SIM: _simg r RR true f_tgt itr_src0 itr_tgt0)
-          (IH: P true f_tgt itr_src0 itr_tgt0),
+          (SIM: _simg r RR TT f_tgt itr_src0 itr_tgt0)
+          (IH: P TT f_tgt itr_src0 itr_tgt0),
           P f_src f_tgt (tau;; itr_src0) (itr_tgt0))
       (TAUR: forall
           f_src f_tgt
           itr_src0 itr_tgt0
           (TAUR: True)
-          (SIM: _simg r RR f_src true itr_src0 itr_tgt0)
-          (IH: P f_src true itr_src0 itr_tgt0),
+          (SIM: _simg r RR f_src TT itr_src0 itr_tgt0)
+          (IH: P f_src TT itr_src0 itr_tgt0),
           P f_src f_tgt (itr_src0) (tau;;itr_tgt0))
       (CHOOSEL: forall
           f_src f_tgt
           X ktr_src0 itr_tgt0
           (CHOOSEL: True)
-          (SIM: exists x, <<SIM: _simg r RR true f_tgt (ktr_src0 x) itr_tgt0>> /\ <<IH: P true f_tgt (ktr_src0 x) itr_tgt0>>),
+          (SIM: exists x, <<SIM: _simg r RR TT f_tgt (ktr_src0 x) itr_tgt0>> /\ <<IH: P TT f_tgt (ktr_src0 x) itr_tgt0>>),
           P f_src f_tgt (trigger (Choose X) >>= ktr_src0) (itr_tgt0))
       (CHOOSER: forall
           f_src f_tgt
           X itr_src0 ktr_tgt0
           (CHOOSER: True)
-          (SIM: forall x, <<SIM: _simg r RR f_src true itr_src0 (ktr_tgt0 x)>> /\ <<IH: P f_src true itr_src0 (ktr_tgt0 x)>>),
+          (SIM: forall x, <<SIM: _simg r RR f_src TT itr_src0 (ktr_tgt0 x)>> /\ <<IH: P f_src TT itr_src0 (ktr_tgt0 x)>>),
           P f_src f_tgt (itr_src0) (trigger (Choose X) >>= ktr_tgt0))
       (TAKEL: forall
           f_src f_tgt
           X ktr_src0 itr_tgt0
           (TAKEL: True)
-          (SIM: forall x, <<SIM: _simg r RR true f_tgt (ktr_src0 x) itr_tgt0>> /\ <<IH: P true f_tgt (ktr_src0 x) itr_tgt0>>),
+          (SIM: forall x, <<SIM: _simg r RR TT f_tgt (ktr_src0 x) itr_tgt0>> /\ <<IH: P TT f_tgt (ktr_src0 x) itr_tgt0>>),
           P f_src f_tgt (trigger (Take X) >>= ktr_src0) (itr_tgt0))
       (TAKER: forall
           f_src f_tgt
           X itr_src0 ktr_tgt0
           (TAKER: True)
-          (SIM: exists x, <<SIM: _simg r RR f_src true itr_src0 (ktr_tgt0 x)>> /\ <<IH: P f_src true itr_src0 (ktr_tgt0 x)>>),
+          (SIM: exists x, <<SIM: _simg r RR f_src TT itr_src0 (ktr_tgt0 x)>> /\ <<IH: P f_src TT itr_src0 (ktr_tgt0 x)>>),
           P f_src f_tgt (itr_src0) (trigger (Take X) >>= ktr_tgt0))
       (PROGRESS: forall
           f_src f_tgt
           itr_src itr_tgt
-          (SIM: r _ _ RR false false itr_src itr_tgt)
-          (SRC: f_src = true)
-          (TGT: f_tgt = true),
+          (SIM: r _ _ RR BB BB itr_src itr_tgt)
+          (SRC: f_src = TT)
+          (TGT: f_tgt = TT),
           P f_src f_tgt itr_src itr_tgt)
   :
     forall f_src f_tgt itr_src itr_tgt
@@ -161,7 +156,7 @@ Proof.
   { eapply PROGRESS; eauto. }
 Qed.
 
-Definition simg: forall R0 R1 (RR: R0 -> R1 -> Prop), bool -> bool -> (itree eventE R0) -> (itree eventE R1) -> Prop := paco7 _simg bot7.
+Definition simg: forall R0 R1 (RR: R0 -> R1 -> Prop), flag -> flag -> (itree eventE R0) -> (itree eventE R1) -> Prop := paco7 _simg bot7.
 
 Lemma simg_mon: monotone7 _simg.
 Proof.
@@ -181,8 +176,8 @@ Hint Resolve cpn7_wcompat: paco.
 
 
 Inductive simg_indC
-          (simg: forall R0 R1 (RR: R0 -> R1 -> Prop), bool -> bool -> (itree eventE R0) -> (itree eventE R1) -> Prop)
-          {R0 R1} (RR: R0 -> R1 -> Prop) (f_src f_tgt: bool): (itree eventE R0) -> (itree eventE R1) -> Prop :=
+          (simg: forall R0 R1 (RR: R0 -> R1 -> Prop), flag -> flag -> (itree eventE R0) -> (itree eventE R1) -> Prop)
+          {R0 R1} (RR: R0 -> R1 -> Prop) (f_src f_tgt: flag): (itree eventE R0) -> (itree eventE R1) -> Prop :=
 | simg_indC_ret
     r_src r_tgt
     (SIM: RR r_src r_tgt)
@@ -190,46 +185,46 @@ Inductive simg_indC
     simg_indC simg RR f_src f_tgt (Ret r_src) (Ret r_tgt)
 | simg_indC_syscall
     ktr_src0 ktr_tgt0 fn varg rvs
-    (SIM: forall x_src x_tgt (EQ: x_src = x_tgt), simg _ _ RR true true (ktr_src0 x_src) (ktr_tgt0 x_tgt))
+    (SIM: forall x_src x_tgt (EQ: x_src = x_tgt), simg _ _ RR TT TT (ktr_src0 x_src) (ktr_tgt0 x_tgt))
   :
     simg_indC simg RR f_src f_tgt (trigger (Syscall fn varg rvs) >>= ktr_src0) (trigger (Syscall fn varg rvs) >>= ktr_tgt0)
 
 | simg_indC_tauL
     itr_src0 itr_tgt0
     (TAUL: True)
-    (SIM: simg _ _ RR true f_tgt itr_src0 itr_tgt0)
+    (SIM: simg _ _ RR TT f_tgt itr_src0 itr_tgt0)
   :
     simg_indC simg RR f_src f_tgt (tau;; itr_src0) (itr_tgt0)
 | simg_indC_tauR
     itr_src0 itr_tgt0
     (TAUR: True)
-    (SIM: simg _ _ RR f_src true itr_src0 itr_tgt0)
+    (SIM: simg _ _ RR f_src TT itr_src0 itr_tgt0)
   :
     simg_indC simg RR f_src f_tgt (itr_src0) (tau;; itr_tgt0)
 
 | simg_indC_chooseL
     X ktr_src0 itr_tgt0
     (CHOOSEL: True)
-    (SIM: exists x, simg _ _ RR true f_tgt (ktr_src0 x) itr_tgt0)
+    (SIM: exists x, simg _ _ RR TT f_tgt (ktr_src0 x) itr_tgt0)
   :
     simg_indC simg RR f_src f_tgt (trigger (Choose X) >>= ktr_src0) (itr_tgt0)
 | simg_indC_chooseR
     X itr_src0 ktr_tgt0
     (CHOOSER: True)
-    (SIM: forall x, simg _ _ RR f_src true itr_src0 (ktr_tgt0 x))
+    (SIM: forall x, simg _ _ RR f_src TT itr_src0 (ktr_tgt0 x))
   :
     simg_indC simg RR f_src f_tgt (itr_src0) (trigger (Choose X) >>= ktr_tgt0)
 
 | simg_indC_takeL
     X ktr_src0 itr_tgt0
     (TAKEL: True)
-    (SIM: forall x, simg _ _ RR true f_tgt (ktr_src0 x) itr_tgt0)
+    (SIM: forall x, simg _ _ RR TT f_tgt (ktr_src0 x) itr_tgt0)
   :
     simg_indC simg RR f_src f_tgt (trigger (Take X) >>= ktr_src0) (itr_tgt0)
 | simg_indC_takeR
     X itr_src0 ktr_tgt0
     (TAKER: True)
-    (SIM: exists x, simg _ _ RR f_src true itr_src0 (ktr_tgt0 x))
+    (SIM: exists x, simg _ _ RR f_src TT itr_src0 (ktr_tgt0 x))
   :
     simg_indC simg RR f_src f_tgt (itr_src0) (trigger (Take X) >>= ktr_tgt0)
 .
@@ -264,7 +259,7 @@ Proof.
 Qed.
 
 Lemma simg_ind R0 R1 (RR: R0 -> R1 -> Prop)
-      (P: bool -> bool -> (itree eventE R0) -> (itree eventE R1) -> Prop)
+      (P: flag -> flag -> (itree eventE R0) -> (itree eventE R1) -> Prop)
       (RET: forall
           f_src f_tgt
           r_src r_tgt
@@ -273,52 +268,52 @@ Lemma simg_ind R0 R1 (RR: R0 -> R1 -> Prop)
       (SYSCALL: forall
           f_src f_tgt
           ktr_src0 ktr_tgt0 fn varg rvs
-          (SIM: forall x_src x_tgt (EQ: x_src = x_tgt), simg RR true true (ktr_src0 x_src) (ktr_tgt0 x_tgt)),
+          (SIM: forall x_src x_tgt (EQ: x_src = x_tgt), simg RR TT TT (ktr_src0 x_src) (ktr_tgt0 x_tgt)),
           P f_src f_tgt (trigger (Syscall fn varg rvs) >>= ktr_src0) (trigger (Syscall fn varg rvs) >>= ktr_tgt0))
       (TAUL: forall
           f_src f_tgt
           itr_src0 itr_tgt0
           (TAUL: True)
-          (SIM: simg RR true f_tgt itr_src0 itr_tgt0)
-          (IH: P true f_tgt itr_src0 itr_tgt0),
+          (SIM: simg RR TT f_tgt itr_src0 itr_tgt0)
+          (IH: P TT f_tgt itr_src0 itr_tgt0),
           P f_src f_tgt (tau;; itr_src0) (itr_tgt0))
       (TAUR: forall
           f_src f_tgt
           itr_src0 itr_tgt0
           (TAUR: True)
-          (SIM: simg RR f_src true itr_src0 itr_tgt0)
-          (IH: P f_src true itr_src0 itr_tgt0),
+          (SIM: simg RR f_src TT itr_src0 itr_tgt0)
+          (IH: P f_src TT itr_src0 itr_tgt0),
           P f_src f_tgt (itr_src0) (tau;;itr_tgt0))
       (CHOOSEL: forall
           f_src f_tgt
           X ktr_src0 itr_tgt0
           (CHOOSEL: True)
-          (SIM: exists x, <<SIM: simg RR true f_tgt (ktr_src0 x) itr_tgt0>> /\ <<IH: P true f_tgt (ktr_src0 x) itr_tgt0>>),
+          (SIM: exists x, <<SIM: simg RR TT f_tgt (ktr_src0 x) itr_tgt0>> /\ <<IH: P TT f_tgt (ktr_src0 x) itr_tgt0>>),
           P f_src f_tgt (trigger (Choose X) >>= ktr_src0) (itr_tgt0))
       (CHOOSER: forall
           f_src f_tgt
           X itr_src0 ktr_tgt0
           (CHOOSER: True)
-          (SIM: forall x, <<SIM: simg RR f_src true itr_src0 (ktr_tgt0 x)>> /\ <<IH: P f_src true itr_src0 (ktr_tgt0 x)>>),
+          (SIM: forall x, <<SIM: simg RR f_src TT itr_src0 (ktr_tgt0 x)>> /\ <<IH: P f_src TT itr_src0 (ktr_tgt0 x)>>),
           P f_src f_tgt (itr_src0) (trigger (Choose X) >>= ktr_tgt0))
       (TAKEL: forall
           f_src f_tgt
           X ktr_src0 itr_tgt0
           (TAKEL: True)
-          (SIM: forall x, <<SIM: simg RR true f_tgt (ktr_src0 x) itr_tgt0>> /\ <<IH: P true f_tgt (ktr_src0 x) itr_tgt0>>),
+          (SIM: forall x, <<SIM: simg RR TT f_tgt (ktr_src0 x) itr_tgt0>> /\ <<IH: P TT f_tgt (ktr_src0 x) itr_tgt0>>),
           P f_src f_tgt (trigger (Take X) >>= ktr_src0) (itr_tgt0))
       (TAKER: forall
           f_src f_tgt
           X itr_src0 ktr_tgt0
           (TAKER: True)
-          (SIM: exists x, <<SIM: simg RR f_src true itr_src0 (ktr_tgt0 x)>> /\ <<IH: P f_src true itr_src0 (ktr_tgt0 x)>>),
+          (SIM: exists x, <<SIM: simg RR f_src TT itr_src0 (ktr_tgt0 x)>> /\ <<IH: P f_src TT itr_src0 (ktr_tgt0 x)>>),
           P f_src f_tgt (itr_src0) (trigger (Take X) >>= ktr_tgt0))
       (PROGRESS: forall
           f_src f_tgt
           itr_src itr_tgt
-          (SIM: simg RR false false itr_src itr_tgt)
-          (SRC: f_src = true)
-          (TGT: f_tgt = true),
+          (SIM: simg RR BB BB itr_src itr_tgt)
+          (SRC: f_src = TT)
+          (TGT: f_tgt = TT),
           P f_src f_tgt itr_src itr_tgt)
   :
     forall f_src f_tgt itr_src itr_tgt
@@ -344,12 +339,12 @@ Hint Unfold simg.
 Hint Resolve simg_mon: paco.
 Hint Resolve cpn7_wcompat: paco.
 
-Variant flagC (r: forall S0 S1 (SS: S0 -> S1 -> Prop), bool -> bool -> (itree eventE S0) -> (itree eventE S1) -> Prop):
-  forall S0 S1 (SS: S0 -> S1 -> Prop), bool -> bool -> (itree eventE S0) -> (itree eventE S1) -> Prop :=
+Variant flagC (r: forall S0 S1 (SS: S0 -> S1 -> Prop), flag -> flag -> (itree eventE S0) -> (itree eventE S1) -> Prop):
+  forall S0 S1 (SS: S0 -> S1 -> Prop), flag -> flag -> (itree eventE S0) -> (itree eventE S1) -> Prop :=
 | flagC_intro
     f_src0 f_src1 f_tgt0 f_tgt1 R0 R1 (RR: R0 -> R1 -> Prop) itr_src itr_tgt
-    (SRC: f_src0 = true -> f_src1 = true)
-    (TGT: f_tgt0 = true -> f_tgt1 = true)
+    (SRC: f_src0 = TT -> f_src1 = TT)
+    (TGT: f_tgt0 = TT -> f_tgt1 = TT)
     (SIM: r _ _ RR f_src0 f_tgt0 itr_src itr_tgt)
   :
     flagC r RR f_src1 f_tgt1 itr_src itr_tgt
@@ -390,8 +385,8 @@ Qed.
 Lemma simg_flag
       r R0 R1 RR itr_src itr_tgt f_src0 f_tgt0 f_src1 f_tgt1
       (SIM: @_simg r R0 R1 RR f_src0 f_tgt0 itr_src itr_tgt)
-      (SRC: f_src0 = true -> f_src1 = true)
-      (TGT: f_tgt0 = true -> f_tgt1 = true)
+      (SRC: f_src0 = TT -> f_src1 = TT)
+      (TGT: f_tgt0 = TT -> f_tgt1 = TT)
   :
     @_simg r R0 R1 RR f_src1 f_tgt1 itr_src itr_tgt.
 Proof.
@@ -408,15 +403,15 @@ Proof.
 Qed.
 
 Lemma simg_progress_flag R0 R1 RR r g itr_src itr_tgt
-      (SIM: gpaco7 _simg (cpn7 _simg) g g R0 R1 RR false false itr_src itr_tgt)
+      (SIM: gpaco7 _simg (cpn7 _simg) g g R0 R1 RR BB BB itr_src itr_tgt)
   :
-    gpaco7 _simg (cpn7 _simg) r g R0 R1 RR true true itr_src itr_tgt.
+    gpaco7 _simg (cpn7 _simg) r g R0 R1 RR TT TT itr_src itr_tgt.
 Proof.
   gstep. econs; eauto.
 Qed.
 
 Lemma simg_flag_down R0 R1 RR r g itr_src itr_tgt f_src f_tgt
-      (SIM: gpaco7 _simg (cpn7 _simg) r g R0 R1 RR false false itr_src itr_tgt)
+      (SIM: gpaco7 _simg (cpn7 _simg) r g R0 R1 RR BB BB itr_src itr_tgt)
   :
     gpaco7 _simg (cpn7 _simg) r g R0 R1 RR f_src f_tgt itr_src itr_tgt.
 Proof.
@@ -424,12 +419,12 @@ Proof.
 Qed.
 
 Lemma simg_bot_flag_up R0 R1 RR st_src st_tgt f_src f_tgt
-      (SIM: @simg R0 R1 RR true true st_src st_tgt)
+      (SIM: @simg R0 R1 RR TT TT st_src st_tgt)
   :
     simg RR f_src f_tgt st_src st_tgt.
 Proof.
-  ginit. remember true in SIM at 1. remember true in SIM at 1.
-  clear Heqb Heqb0. revert st_src st_tgt f_src f_tgt b b0 SIM.
+  ginit. remember TT in SIM at 1. remember TT in SIM at 1.
+  clear Heqf Heqf0. revert st_src st_tgt f_src f_tgt f f0 SIM.
   gcofix CIH. i. revert f_src f_tgt.
   induction SIM using simg_ind.
   { guclo simg_indC_spec. econs 1; eauto. }
@@ -446,8 +441,8 @@ Proof.
 Qed.
 
 
-Variant bindR (r s: forall S0 S1 (SS: S0 -> S1 -> Prop), bool -> bool -> (itree eventE S0) -> (itree eventE S1) -> Prop):
-  forall S0 S1 (SS: S0 -> S1 -> Prop), bool -> bool -> (itree eventE S0) -> (itree eventE S1) -> Prop :=
+Variant bindR (r s: forall S0 S1 (SS: S0 -> S1 -> Prop), flag -> flag -> (itree eventE S0) -> (itree eventE S1) -> Prop):
+  forall S0 S1 (SS: S0 -> S1 -> Prop), flag -> flag -> (itree eventE S0) -> (itree eventE S1) -> Prop :=
 | bindR_intro
     f_src f_tgt
 
@@ -457,7 +452,7 @@ Variant bindR (r s: forall S0 S1 (SS: S0 -> S1 -> Prop), bool -> bool -> (itree 
 
     S0 S1 SS
     (k_src: ktree eventE R0 S0) (k_tgt: ktree eventE R1 S1)
-    (SIMK: forall vret_src vret_tgt (SIM: RR vret_src vret_tgt), s _ _ SS false false (k_src vret_src) (k_tgt vret_tgt))
+    (SIMK: forall vret_src vret_tgt (SIM: RR vret_src vret_tgt), s _ _ SS BB BB (k_src vret_src) (k_tgt vret_tgt))
   :
     bindR r s SS f_src f_tgt (ITree.bind i_src k_src) (ITree.bind i_tgt k_tgt)
 .
@@ -634,15 +629,15 @@ Context {CONFS CONFT: EMSConfig}.
 Hypothesis (FINSAME: (@finalize CONFS) = (@finalize CONFT)).
 
 Theorem adequacy_global_itree itr_src itr_tgt
-        (SIM: simg eq false false itr_src itr_tgt)
+        (SIM: simg eq BB BB itr_src itr_tgt)
   :
     Beh.of_program (@ModSem.compile_itree CONFT itr_tgt)
     <1=
     Beh.of_program (@ModSem.compile_itree CONFS itr_src).
 Proof.
   unfold Beh.of_program. ss.
-  remember false as o_src0 in SIM at 1.
-  remember false as o_tgt0 in SIM at 1. clear Heqo_src0 Heqo_tgt0.
+  remember BB as o_src0 in SIM at 1.
+  remember BB as o_tgt0 in SIM at 1. clear Heqo_src0 Heqo_tgt0.
   i. eapply adequacy_aux; et.
   instantiate (1:=o_tgt0). instantiate (1:=o_src0). clear x0 PR.
   generalize itr_tgt at 1 as md_tgt.
@@ -691,8 +686,8 @@ Let ms_src: ModSem.t := md_src.(Mod.enclose).
 Let ms_tgt: ModSem.t := md_tgt.(Mod.enclose).
 
 Section ADEQUACY.
-(* Hypothesis (SIM: simg eq false false (@ModSem.initial_itr ms_src CONFS ) (@ModSem.initial_itr ms_tgt CONFT )). *)
-Hypothesis (SIM: simg eq false false (@ModSem.initial_itr ms_src CONFS (Some (Mod.wf md_src))) (@ModSem.initial_itr ms_tgt CONFT (Some (Mod.wf md_tgt)))).
+(* Hypothesis (SIM: simg eq BB BB (@ModSem.initial_itr ms_src CONFS ) (@ModSem.initial_itr ms_tgt CONFT )). *)
+Hypothesis (SIM: simg eq BB BB (@ModSem.initial_itr ms_src CONFS (Some (Mod.wf md_src))) (@ModSem.initial_itr ms_tgt CONFT (Some (Mod.wf md_tgt)))).
 
 
 Theorem adequacy_global: Beh.of_program (@Mod.compile _ CONFT md_tgt) <1= Beh.of_program (@Mod.compile _ CONFS md_src).
@@ -714,8 +709,8 @@ Hint Resolve sim_indC_mon: paco.
 
 
 Variant _simg_safe
-          (simg: forall R0 R1 (RR: R0 -> R1 -> Prop), bool -> bool -> (itree eventE R0) -> (itree eventE R1) -> Prop)
-          {R0 R1} (RR: R0 -> R1 -> Prop) (f_src f_tgt: bool): (itree eventE R0) -> (itree eventE R1) -> Prop :=
+          (simg: forall R0 R1 (RR: R0 -> R1 -> Prop), flag -> flag -> (itree eventE R0) -> (itree eventE R1) -> Prop)
+          {R0 R1} (RR: R0 -> R1 -> Prop) (f_src f_tgt: flag): (itree eventE R0) -> (itree eventE R1) -> Prop :=
 | simg_safe_ret
     r_src r_tgt
     (SIM: RR r_src r_tgt)
@@ -723,34 +718,34 @@ Variant _simg_safe
     _simg_safe simg RR f_src f_tgt (Ret r_src) (Ret r_tgt)
 | simg_safe_syscall
     ktr_src0 ktr_tgt0 fn varg rvs
-    (SIM: forall x_src x_tgt (EQ: x_src = x_tgt), simg _ _ RR true true (ktr_src0 x_src) (ktr_tgt0 x_tgt))
+    (SIM: forall x_src x_tgt (EQ: x_src = x_tgt), simg _ _ RR TT TT (ktr_src0 x_src) (ktr_tgt0 x_tgt))
   :
     _simg_safe simg RR f_src f_tgt (trigger (Syscall fn varg rvs) >>= ktr_src0) (trigger (Syscall fn varg rvs) >>= ktr_tgt0)
 
 | simg_safe_tauL
     itr_src0 itr_tgt0
     (TAUL: True)
-    (SIM: simg _ _ RR true f_tgt itr_src0 itr_tgt0)
+    (SIM: simg _ _ RR TT f_tgt itr_src0 itr_tgt0)
   :
     _simg_safe simg RR f_src f_tgt (tau;; itr_src0) (itr_tgt0)
 | simg_safe_tauR
     itr_src0 itr_tgt0
     (TAUR: True)
-    (SIM: simg _ _ RR f_src true itr_src0 itr_tgt0)
+    (SIM: simg _ _ RR f_src TT itr_src0 itr_tgt0)
   :
     _simg_safe simg RR f_src f_tgt (itr_src0) (tau;; itr_tgt0)
 
 | simg_safe_chooseR
     X itr_src0 ktr_tgt0
     (CHOOSER: True)
-    (SIM: forall x, simg _ _ RR f_src true itr_src0 (ktr_tgt0 x))
+    (SIM: forall x, simg _ _ RR f_src TT itr_src0 (ktr_tgt0 x))
   :
     _simg_safe simg RR f_src f_tgt (itr_src0) (trigger (Choose X) >>= ktr_tgt0)
 
 | simg_safe_takeL
     X ktr_src0 itr_tgt0
     (TAKEL: True)
-    (SIM: forall x, simg _ _ RR true f_tgt (ktr_src0 x) itr_tgt0)
+    (SIM: forall x, simg _ _ RR TT f_tgt (ktr_src0 x) itr_tgt0)
   :
     _simg_safe simg RR f_src f_tgt (trigger (Take X) >>= ktr_src0) (itr_tgt0)
 .
