ems/SimModSem.v
@@ -15,6 +15,8 @@ From ExtLib Require Import
      Structures.Maps
      Data.Map.FMapAList.
 Require Import Any.
+Require Import SimSTS.
+Require Import SimGlobal.
 
 Set Implicit Arguments.
 
@@ -32,9 +34,11 @@ Section SIM.
 
 
 
-  Inductive _sim_itree (sim_itree: forall (R_src R_tgt: Type) (RR: st_local -> st_local -> R_src -> R_tgt -> Prop), bool -> bool -> world -> st_local * itree Es R_src -> st_local * itree Es R_tgt -> Prop)
+
+
+  Inductive _sim_itree (sim_itree: forall (R_src R_tgt: Type) (RR: st_local -> st_local -> R_src -> R_tgt -> Prop), flag -> flag -> world -> st_local * itree Es R_src -> st_local * itree Es R_tgt -> Prop)
           {R_src R_tgt} (RR: st_local -> st_local -> R_src -> R_tgt -> Prop)
-    : bool -> bool -> world -> st_local * itree Es R_src -> st_local * itree Es R_tgt -> Prop :=
+    : flag -> flag -> world -> st_local * itree Es R_src -> st_local * itree Es R_tgt -> Prop :=
   | sim_itree_ret
       i_src0 i_tgt0 w0 st_src0 st_tgt0
       v_src v_tgt
@@ -47,7 +51,7 @@ Section SIM.
       fn varg k_src k_tgt
       (WF: wf w0 (st_src0, st_tgt0))
       (K: forall w1 vret st_src1 st_tgt1 (WLE: le w0 w1) (WF: wf w1 (st_src1, st_tgt1)),
-          sim_itree _ _ RR true true w (st_src1, k_src vret) (st_tgt1, k_tgt vret))
+          sim_itree _ _ RR TT TT w (st_src1, k_src vret) (st_tgt1, k_tgt vret))
     :
       _sim_itree sim_itree RR i_src0 i_tgt0 w (st_src0, trigger (Call fn varg) >>= k_src)
                  (st_tgt0, trigger (Call fn varg) >>= k_tgt)
@@ -56,7 +60,7 @@ Section SIM.
       i_src0 i_tgt0 w0 st_src0 st_tgt0
       fn varg rvs k_src k_tgt
       (K: forall vret,
-          sim_itree _ _ RR true true w0 (st_src0, k_src vret) (st_tgt0, k_tgt vret))
+          sim_itree _ _ RR TT TT w0 (st_src0, k_src vret) (st_tgt0, k_tgt vret))
     :
       _sim_itree sim_itree RR i_src0 i_tgt0 w0 (st_src0, trigger (Syscall fn varg rvs) >>= k_src)
                  (st_tgt0, trigger (Syscall fn varg rvs) >>= k_tgt)
@@ -66,7 +70,7 @@ Section SIM.
       f fn varg k_src i_tgt
       (FUN: alist_find fn fl_src = Some f)
       (* (IN: In (fn, f) fl_src ) *)
-      (K: _sim_itree sim_itree RR true i_tgt0 w (st_src, (f varg) >>= k_src) (st_tgt, i_tgt))
+      (K: _sim_itree sim_itree RR TT i_tgt0 w (st_src, (f varg) >>= k_src) (st_tgt, i_tgt))
     :
       _sim_itree sim_itree RR i_src0 i_tgt0 w (st_src, trigger (Call fn varg) >>= k_src)
                  (st_tgt, i_tgt)
@@ -76,7 +80,7 @@ Section SIM.
       f fn varg i_src k_tgt
       (FUN: alist_find fn fl_tgt = Some f)
       (* (IN: In (fn, f) fl_tgt ) *)
-      (K: _sim_itree sim_itree RR i_src0 true w (st_src, i_src) (st_tgt, (f varg) >>= k_tgt))
+      (K: _sim_itree sim_itree RR i_src0 TT w (st_src, i_src) (st_tgt, (f varg) >>= k_tgt))
     :
       _sim_itree sim_itree RR i_src0 i_tgt0 w (st_src, i_src)
                  (st_tgt, trigger (Call fn varg) >>= k_tgt)
@@ -84,21 +88,21 @@ Section SIM.
   | sim_itree_tau_src
       i_src0 i_tgt0 w0 (st_src0: st_local) (st_tgt0: st_local)
       i_src i_tgt
-      (K: _sim_itree sim_itree RR true i_tgt0 w0 (st_src0, i_src) (st_tgt0, i_tgt))
+      (K: _sim_itree sim_itree RR TT i_tgt0 w0 (st_src0, i_src) (st_tgt0, i_tgt))
     :
       _sim_itree sim_itree RR i_src0 i_tgt0 w0 (st_src0, tau;; i_src) (st_tgt0, i_tgt)
 
   | sim_itree_tau_tgt
       i_src0 i_tgt0 w0 (st_src0: st_local) (st_tgt0: st_local)
       i_src i_tgt
-      (K: _sim_itree sim_itree RR i_src0 true w0 (st_src0, i_src) (st_tgt0, i_tgt))
+      (K: _sim_itree sim_itree RR i_src0 TT w0 (st_src0, i_src) (st_tgt0, i_tgt))
     :
       _sim_itree sim_itree RR i_src0 i_tgt0 w0 (st_src0, i_src) (st_tgt0, tau;; i_tgt)
 
   | sim_itree_choose_src
       i_src0 i_tgt0 w0 (st_src0: st_local) (st_tgt0: st_local)
       X k_src i_tgt
-      (K: exists (x: X), _sim_itree sim_itree RR true i_tgt0 w0 (st_src0, k_src x) (st_tgt0, i_tgt))
+      (K: exists (x: X), _sim_itree sim_itree RR TT i_tgt0 w0 (st_src0, k_src x) (st_tgt0, i_tgt))
     :
       _sim_itree sim_itree RR i_src0 i_tgt0 w0 (st_src0, trigger (Choose X) >>= k_src)
                  (st_tgt0, i_tgt)
@@ -106,7 +110,7 @@ Section SIM.
   | sim_itree_choose_tgt
       i_src0 i_tgt0 w0 (st_src0: st_local) (st_tgt0: st_local)
       X i_src k_tgt
-      (K: forall (x: X), _sim_itree sim_itree RR i_src0 true w0 (st_src0, i_src) (st_tgt0, k_tgt x))
+      (K: forall (x: X), _sim_itree sim_itree RR i_src0 TT w0 (st_src0, i_src) (st_tgt0, k_tgt x))
     :
       _sim_itree sim_itree RR i_src0 i_tgt0 w0 (st_src0, i_src)
                  (st_tgt0, trigger (Choose X) >>= k_tgt)
@@ -114,7 +118,7 @@ Section SIM.
   | sim_itree_take_src
       i_src0 i_tgt0 w0 (st_src0: st_local) (st_tgt0: st_local)
       X k_src i_tgt
-      (K: forall (x: X), _sim_itree sim_itree RR true i_tgt0 w0 (st_src0, k_src x) (st_tgt0, i_tgt))
+      (K: forall (x: X), _sim_itree sim_itree RR TT i_tgt0 w0 (st_src0, k_src x) (st_tgt0, i_tgt))
     :
       _sim_itree sim_itree RR i_src0 i_tgt0 w0 (st_src0, trigger (Take X) >>= k_src)
                  (st_tgt0, i_tgt)
@@ -122,7 +126,7 @@ Section SIM.
   | sim_itree_take_tgt
       i_src0 i_tgt0 w0 (st_src0: st_local) (st_tgt0: st_local)
       X i_src k_tgt
-      (K: exists (x: X), _sim_itree sim_itree RR i_src0 true w0 (st_src0, i_src) (st_tgt0, k_tgt x))
+      (K: exists (x: X), _sim_itree sim_itree RR i_src0 TT w0 (st_src0, i_src) (st_tgt0, k_tgt x))
     :
       _sim_itree sim_itree RR i_src0 i_tgt0 w0 (st_src0, i_src)
                  (st_tgt0, trigger (Take X) >>= k_tgt)
@@ -131,7 +135,7 @@ Section SIM.
       i_src0 i_tgt0 w0 (st_src0: st_local) (st_tgt0: st_local)
       X k_src i_tgt
       (run: st_local -> st_local * X )
-      (K: _sim_itree sim_itree RR true i_tgt0 w0 (fst (run st_src0), k_src (snd (run st_src0))) (st_tgt0, i_tgt))
+      (K: _sim_itree sim_itree RR TT i_tgt0 w0 (fst (run st_src0), k_src (snd (run st_src0))) (st_tgt0, i_tgt))
     :
       _sim_itree sim_itree RR i_src0 i_tgt0 w0 (st_src0, trigger (SUpdate run) >>= k_src) (st_tgt0, i_tgt)  
 
@@ -139,17 +143,59 @@ Section SIM.
       i_src0 i_tgt0 w0 (st_src0: st_local) (st_tgt0: st_local)
       X i_src k_tgt
       (run: st_local -> st_local * X )
-      (K: _sim_itree sim_itree RR i_src0 true w0 (st_src0, i_src) (fst (run st_tgt0), k_tgt (snd (run st_tgt0))))
+      (K: _sim_itree sim_itree RR i_src0 TT w0 (st_src0, i_src) (fst (run st_tgt0), k_tgt (snd (run st_tgt0))))
     :
       _sim_itree sim_itree RR i_src0 i_tgt0 w0 (st_src0, i_src) (st_tgt0, trigger (SUpdate run) >>= k_tgt)
 
-  | sim_itree_progress
-      i_src0 i_tgt0 w0 (st_src0: st_local) (st_tgt0: st_local) i_src i_tgt
-      (SIM: sim_itree _ _ RR false false w0 (st_src0, i_src) (st_tgt0, i_tgt))
-      (SRC: i_src0 = true)
-      (TGT: i_tgt0 = true)
+  | sim_itree_yield_tgt
+      i_src0 i_tgt0 w w0 st_src0 st_tgt0
+      k_src k_tgt
+      (WF: wf w0 (st_src0, st_tgt0))
+      (K: forall w1 st_tgt1 (WLE: le w0 w1) (WF: wf w1 (st_src0, st_tgt1)),
+        _sim_itree sim_itree RR i_src0 YY w (st_src0, trigger Yield >>= k_src) (st_tgt1, k_tgt tt))
     :
-      _sim_itree sim_itree RR true true w0 (st_src0, i_src) (st_tgt0, i_tgt)
+      _sim_itree sim_itree RR i_src0 i_tgt0 w (st_src0, trigger Yield >>= k_src)
+                 (st_tgt0, trigger Yield >>= k_tgt)
+
+  | sim_itree_yield_src
+      i_src0 i_tgt0 w0 st_src0 st_tgt0
+      k_src i_tgt
+      st_src1
+      (K: _sim_itree sim_itree RR YY i_tgt0 w0 (st_src1, k_src tt) (st_tgt0, i_tgt))
+    :
+      _sim_itree sim_itree RR i_src0 i_tgt0 w0 (st_src0, (trigger Yield) >>= k_src) (st_tgt0, i_tgt)
+  | sim_itree_spawn
+      i_src0 i_tgt0 w w0 st_src0 st_tgt0
+      fn varg k_src k_tgt
+      (WF: wf w0 (st_src0, st_tgt0))
+      (K: forall w1 vret st_src1 st_tgt1 (WLE: le w0 w1) (WF: wf w1 (st_src1, st_tgt1)),
+          sim_itree _ _ RR YY YY w (st_src1, k_src vret) (st_tgt1, k_tgt vret))
+    :
+      _sim_itree sim_itree RR i_src0 i_tgt0 w (st_src0, trigger (Spawn fn varg) >>= k_src)
+                 (st_tgt0, trigger (Spawn fn varg) >>= k_tgt)
+  | sim_itree_progress
+      i_flag w0 (st_src0: st_local) (st_tgt0: st_local) i_src i_tgt
+      (SIM: sim_itree _ _ RR BB BB w0 (st_src0, i_src) (st_tgt0, i_tgt))
+      (FLAG: i_flag = TT \/ i_flag = YY)
+    :
+      _sim_itree sim_itree RR i_flag i_flag w0 (st_src0, i_src) (st_tgt0, i_tgt)      
+
+  (* | sim_itree_progress_t
+      i_src0 i_tgt0 w0 (st_src0: st_local) (st_tgt0: st_local) i_src i_tgt
+      (SIM: sim_itree _ _ RR BB BB w0 (st_src0, i_src) (st_tgt0, i_tgt))
+      (SRC: i_src0 = TT)
+      (TGT: i_tgt0 = TT)
+    :
+      _sim_itree sim_itree RR TT TT w0 (st_src0, i_src) (st_tgt0, i_tgt)
+
+  | sim_itree_progress_y
+      i_src0 i_tgt0 w0 (st_src0: st_local) (st_tgt0: st_local) i_src i_tgt
+      (SIM: sim_itree _ _ RR BB BB w0 (st_src0, i_src) (st_tgt0, i_tgt))
+      (SRC: i_src0 = YY)
+      (TGT: i_tgt0 = YY)
+    :
+      _sim_itree sim_itree RR YY YY w0 (st_src0, i_src) (st_tgt0, i_tgt)       *)
+
   .
 
   Definition lift_rel {R_src R_tgt} (w0: world) (RR: R_src -> R_tgt -> Prop)
@@ -158,9 +204,9 @@ Section SIM.
       (<<WLE: le w0 w1 >> /\ <<WF: wf w1 (st_src0, st_tgt0) >> /\ <<RET: ret_src = ret_tgt >>).
 
   Lemma _sim_itree_ind2 (sim_itree: forall (R_src R_tgt: Type) 
-                                    (RR: st_local -> st_local -> R_src -> R_tgt -> Prop), bool -> bool -> world -> st_local * itree Es R_src -> st_local * itree Es R_tgt -> Prop)
+                                    (RR: st_local -> st_local -> R_src -> R_tgt -> Prop), flag -> flag -> world -> st_local * itree Es R_src -> st_local * itree Es R_tgt -> Prop)
         {R_src R_tgt} (RR: st_local -> st_local -> R_src -> R_tgt -> Prop)
-        (P: bool -> bool -> world -> st_local * itree Es R_src -> st_local * itree Es R_tgt -> Prop)
+        (P: flag -> flag -> world -> st_local * itree Es R_src -> st_local * itree Es R_tgt -> Prop)
         (RET: forall
             i_src0 i_tgt0 w0 st_src0 st_tgt0
             v_src v_tgt
@@ -171,14 +217,14 @@ Section SIM.
             fn varg k_src k_tgt
             (WF: wf w0 (st_src0, st_tgt0))
             (K: forall w1 vret st_src1 st_tgt1 (WLE: le w0 w1) (WF: wf w1 (st_src1, st_tgt1)),
-                sim_itree _ _ RR true true w (st_src1, k_src vret) (st_tgt1, k_tgt vret)),
+                sim_itree _ _ RR TT TT w (st_src1, k_src vret) (st_tgt1, k_tgt vret)),
             P i_src0 i_tgt0 w (st_src0, trigger (Call fn varg) >>= k_src)
               (st_tgt0, trigger (Call fn varg) >>= k_tgt))
         (SYSCALL: forall
             i_src0 i_tgt0 w0 (st_src0: st_local) (st_tgt0: st_local)
             fn varg rvs k_src k_tgt
             (K: forall vret,
-                sim_itree _ _ RR true true w0 (st_src0, k_src vret) (st_tgt0, k_tgt vret)),
+                sim_itree _ _ RR TT TT w0 (st_src0, k_src vret) (st_tgt0, k_tgt vret)),
             P i_src0 i_tgt0 w0 (st_src0, trigger (Syscall fn varg rvs) >>= k_src)
               (st_tgt0, trigger (Syscall fn varg rvs) >>= k_tgt))
         (INLINESRC: forall
@@ -186,8 +232,8 @@ Section SIM.
             f fn varg k_src i_tgt
             (FUN: alist_find fn fl_src = Some f)
             (* (IN: In (fn, f) fl_src )  *)
-            (K: _sim_itree sim_itree RR true i_tgt0 w (st_src, (f varg) >>= k_src) (st_tgt, i_tgt))
-            (IH: P true i_tgt0 w (st_src, (f varg) >>= k_src) (st_tgt, i_tgt)),
+            (K: _sim_itree sim_itree RR TT i_tgt0 w (st_src, (f varg) >>= k_src) (st_tgt, i_tgt))
+            (IH: P TT i_tgt0 w (st_src, (f varg) >>= k_src) (st_tgt, i_tgt)),
             P i_src0 i_tgt0 w (st_src, trigger (Call fn varg) >>= k_src)
               (st_tgt, i_tgt))
         (INLINETGT: forall
@@ -195,66 +241,89 @@ Section SIM.
             f fn varg i_src k_tgt
             (FUN: alist_find fn fl_tgt = Some f)
             (* (IN: In (fn, f) fl_tgt )  *)
-            (K: _sim_itree sim_itree RR i_src0 true w (st_src, i_src) (st_tgt, (f varg) >>= k_tgt))
-            (IH: P i_src0 true w (st_src, i_src) (st_tgt, (f varg) >>= k_tgt)),
+            (K: _sim_itree sim_itree RR i_src0 TT w (st_src, i_src) (st_tgt, (f varg) >>= k_tgt))
+            (IH: P i_src0 TT w (st_src, i_src) (st_tgt, (f varg) >>= k_tgt)),
             P i_src0 i_tgt0 w (st_src, i_src)
               (st_tgt, trigger (Call fn varg) >>= k_tgt)) 
         (TAUSRC: forall
             i_src0 i_tgt0 w0 (st_src0: st_local) (st_tgt0: st_local)
             i_src i_tgt
-            (K: _sim_itree sim_itree RR true i_tgt0 w0 (st_src0, i_src) (st_tgt0, i_tgt))
-            (IH: P true i_tgt0 w0 (st_src0, i_src) (st_tgt0, i_tgt)),
+            (K: _sim_itree sim_itree RR TT i_tgt0 w0 (st_src0, i_src) (st_tgt0, i_tgt))
+            (IH: P TT i_tgt0 w0 (st_src0, i_src) (st_tgt0, i_tgt)),
             P i_src0 i_tgt0 w0 (st_src0, tau;; i_src) (st_tgt0, i_tgt))
         (TAUTGT: forall
             i_src0 i_tgt0 w0 (st_src0: st_local) (st_tgt0: st_local)
             i_src i_tgt
-            (K: _sim_itree sim_itree RR i_src0 true w0 (st_src0, i_src) (st_tgt0, i_tgt))
-            (IH: P i_src0 true w0 (st_src0, i_src) (st_tgt0, i_tgt)),
+            (K: _sim_itree sim_itree RR i_src0 TT w0 (st_src0, i_src) (st_tgt0, i_tgt))
+            (IH: P i_src0 TT w0 (st_src0, i_src) (st_tgt0, i_tgt)),
             P i_src0 i_tgt0 w0 (st_src0, i_src) (st_tgt0, tau;; i_tgt))
         (CHOOSESRC: forall
             i_src0 i_tgt0 w0 (st_src0: st_local) (st_tgt0: st_local)
             X k_src i_tgt
-            (K: exists (x: X), <<SIM: _sim_itree sim_itree RR true i_tgt0 w0 (st_src0, k_src x) (st_tgt0, i_tgt)>> /\ <<IH: P true i_tgt0 w0 (st_src0, k_src x) (st_tgt0, i_tgt)>>),
+            (K: exists (x: X), <<SIM: _sim_itree sim_itree RR TT i_tgt0 w0 (st_src0, k_src x) (st_tgt0, i_tgt)>> /\ <<IH: P TT i_tgt0 w0 (st_src0, k_src x) (st_tgt0, i_tgt)>>),
             P i_src0 i_tgt0 w0 (st_src0, trigger (Choose X) >>= k_src)
               (st_tgt0, i_tgt))
         (CHOOSETGT: forall
             i_src0 i_tgt0 w0 (st_src0: st_local) (st_tgt0: st_local)
             X i_src k_tgt
-            (K: forall (x: X), <<SIMH: _sim_itree sim_itree RR i_src0 true w0 (st_src0, i_src) (st_tgt0, k_tgt x)>> /\ <<IH: P i_src0 true w0 (st_src0, i_src) (st_tgt0, k_tgt x)>>),
+            (K: forall (x: X), <<SIMH: _sim_itree sim_itree RR i_src0 TT w0 (st_src0, i_src) (st_tgt0, k_tgt x)>> /\ <<IH: P i_src0 TT w0 (st_src0, i_src) (st_tgt0, k_tgt x)>>),
             P i_src0 i_tgt0 w0 (st_src0, i_src)
               (st_tgt0, trigger (Choose X) >>= k_tgt))
         (TAKESRC: forall
             i_src0 i_tgt0 w0 (st_src0: st_local) (st_tgt0: st_local)
             X k_src i_tgt
-            (K: forall (x: X), <<SIM: _sim_itree sim_itree RR true i_tgt0 w0 (st_src0, k_src x) (st_tgt0, i_tgt)>> /\ <<IH: P true i_tgt0 w0 (st_src0, k_src x) (st_tgt0, i_tgt)>>),
+            (K: forall (x: X), <<SIM: _sim_itree sim_itree RR TT i_tgt0 w0 (st_src0, k_src x) (st_tgt0, i_tgt)>> /\ <<IH: P TT i_tgt0 w0 (st_src0, k_src x) (st_tgt0, i_tgt)>>),
             P i_src0 i_tgt0 w0 (st_src0, trigger (Take X) >>= k_src)
               (st_tgt0, i_tgt))
         (TAKETGT: forall
             i_src0 i_tgt0 w0 (st_src0: st_local) (st_tgt0: st_local)
             X i_src k_tgt
-            (K: exists (x: X), <<SIM:_sim_itree sim_itree RR i_src0 true w0 (st_src0, i_src) (st_tgt0, k_tgt x)>> /\ <<IH: P i_src0 true w0 (st_src0, i_src) (st_tgt0, k_tgt x)>>),
+            (K: exists (x: X), <<SIM:_sim_itree sim_itree RR i_src0 TT w0 (st_src0, i_src) (st_tgt0, k_tgt x)>> /\ <<IH: P i_src0 TT w0 (st_src0, i_src) (st_tgt0, k_tgt x)>>),
             P i_src0 i_tgt0 w0 (st_src0, i_src)
               (st_tgt0, trigger (Take X) >>= k_tgt))
         (SUPDATESRC: forall
             i_src0 i_tgt0 w0 (st_src0: st_local) (st_tgt0: st_local)
             X k_src i_tgt
             (run: st_local -> st_local * X )
-            (K: _sim_itree sim_itree RR true i_tgt0 w0 (fst (run st_src0), k_src (snd (run st_src0))) (st_tgt0, i_tgt))
-            (IH: P true i_tgt0 w0 (fst (run st_src0), k_src (snd (run st_src0))) (st_tgt0, i_tgt)),
+            (K: _sim_itree sim_itree RR TT i_tgt0 w0 (fst (run st_src0), k_src (snd (run st_src0))) (st_tgt0, i_tgt))
+            (IH: P TT i_tgt0 w0 (fst (run st_src0), k_src (snd (run st_src0))) (st_tgt0, i_tgt)),
             P i_src0 i_tgt0 w0 (st_src0, trigger (SUpdate run) >>= k_src) (st_tgt0, i_tgt))
         (SUPDATETGT: forall
             i_src0 i_tgt0 w0 (st_src0: st_local) (st_tgt0: st_local)
             X i_src k_tgt
             (run: st_local -> st_local * X )
-            (K: _sim_itree sim_itree RR i_src0 true w0 (st_src0, i_src) (fst (run st_tgt0), k_tgt (snd (run st_tgt0))))
-            (IH: P i_src0 true w0 (st_src0, i_src) (fst (run st_tgt0), k_tgt (snd (run st_tgt0)))),
+            (K: _sim_itree sim_itree RR i_src0 TT w0 (st_src0, i_src) (fst (run st_tgt0), k_tgt (snd (run st_tgt0))))
+            (IH: P i_src0 TT w0 (st_src0, i_src) (fst (run st_tgt0), k_tgt (snd (run st_tgt0)))),
             P i_src0 i_tgt0 w0 (st_src0, i_src) (st_tgt0, trigger (SUpdate run) >>= k_tgt))
+        (YIELDTGT: forall
+            i_src0 i_tgt0 w w0 st_src0 st_tgt0
+            k_src k_tgt
+            (WF: wf w0 (st_src0, st_tgt0))
+            (K: forall w1 st_tgt1 (WLE: le w0 w1) (WF: wf w1 (st_src0, st_tgt1)),
+              << SIMH: _sim_itree sim_itree RR i_src0 YY w (st_src0, trigger Yield >>= k_src) (st_tgt1, k_tgt tt) >> 
+              /\ << IH: P i_src0 YY w (st_src0, trigger Yield >>= k_src) (st_tgt1, k_tgt tt) >> ),
+            P i_src0 i_tgt0 w (st_src0, trigger Yield >>= k_src) (st_tgt0, trigger Yield >>= k_tgt ))
+        (YIELDSRC: forall
+            i_src0 i_tgt0 w0 st_src0 st_tgt0
+            k_src i_tgt
+            st_src1
+            (K: _sim_itree sim_itree RR YY i_tgt0 w0 (st_src1, k_src tt) (st_tgt0, i_tgt))
+            (IH: P YY i_tgt0 w0 (st_src1, k_src tt) (st_tgt0, i_tgt)),
+            P i_src0 i_tgt0 w0 (st_src0, trigger Yield >>= k_src) (st_tgt0, i_tgt))
+        (SPAWN: forall
+            i_src0 i_tgt0 w w0 st_src0 st_tgt0
+            fn varg k_src k_tgt
+            (WF: wf w0 (st_src0, st_tgt0))
+            (K: forall w1 vret st_src1 st_tgt1 (WLE: le w0 w1) (WF: wf w1 (st_src1, st_tgt1)),
+                sim_itree _ _ RR YY YY w (st_src1, k_src vret) (st_tgt1, k_tgt vret)),
+            P i_src0 i_tgt0 w (st_src0, trigger (Spawn fn varg) >>= k_src)
+              (st_tgt0, trigger (Spawn fn varg) >>= k_tgt))
         (PROGRESS: forall
-            i_src0 i_tgt0 w0 (st_src0: st_local) (st_tgt0: st_local) i_src i_tgt
-            (SIM: sim_itree _ _ RR false false w0 (st_src0, i_src) (st_tgt0, i_tgt))
-            (SRC: i_src0 = true)
-            (TGT: i_tgt0 = true),
-            P true true w0 (st_src0, i_src) (st_tgt0, i_tgt))
+            i_flag w0 (st_src0: st_local) (st_tgt0: st_local) i_src i_tgt
+            (SIM: sim_itree _ _ RR BB BB w0 (st_src0, i_src) (st_tgt0, i_tgt))
+            (FLAG: i_flag = TT \/ i_flag = YY),
+            P i_flag i_flag w0 (st_src0, i_src) (st_tgt0, i_tgt))
+    
     :
       forall i_src0 i_tgt0 w0 st_src st_tgt
              (SIM: _sim_itree sim_itree RR i_src0 i_tgt0 w0 st_src st_tgt),
@@ -274,8 +343,10 @@ Section SIM.
     { eapply TAKETGT; eauto. des. esplits; eauto. }
     { eapply SUPDATESRC; eauto. }
     { eapply SUPDATETGT; eauto. }
+    { eapply YIELDTGT; et. esplits; et. }
+    { eapply YIELDSRC; et. }
+    { eapply SPAWN; et. }
     { eapply PROGRESS; eauto. }
-
   Qed.
 
   Definition sim_itree o_src o_tgt w0 : relation _ :=
@@ -284,6 +355,7 @@ Section SIM.
   Lemma sim_itree_mon: monotone8 _sim_itree.
   Proof.
     ii. induction IN using _sim_itree_ind2; try (by des; econs; ss; et).
+    - econs; ss; et. ii. exploit K; et. i; des. esplits; et.
     - econs; ss; et. ii. exploit K; et. i; des. esplits; et.
     - econs; ss; et. ii. exploit K; et. i; des. esplits; et.
   Qed.
@@ -295,7 +367,7 @@ Section SIM.
 
   Lemma sim_itree_ind
         R_src R_tgt (RR: st_local -> st_local -> R_src -> R_tgt -> Prop) 
-        (P: bool -> bool -> world -> st_local * itree Es R_src -> st_local * itree Es R_tgt -> Prop)
+        (P: flag -> flag -> world -> st_local * itree Es R_src -> st_local * itree Es R_tgt -> Prop)
         (RET: forall
             i_src0 i_tgt0 w0 st_src0 st_tgt0
             v_src v_tgt
@@ -306,14 +378,14 @@ Section SIM.
             fn varg k_src k_tgt
             (WF: wf w0 (st_src0, st_tgt0))
             (K: forall w1 vret st_src1 st_tgt1 (WLE: le w0 w1) (WF: wf w1 (st_src1, st_tgt1)),
-                paco8 _sim_itree bot8 _ _ RR true true w (st_src1, k_src vret) (st_tgt1, k_tgt vret)),
+                paco8 _sim_itree bot8 _ _ RR TT TT w (st_src1, k_src vret) (st_tgt1, k_tgt vret)),
             P i_src0 i_tgt0 w (st_src0, trigger (Call fn varg) >>= k_src)
               (st_tgt0, trigger (Call fn varg) >>= k_tgt))
         (SYSCALL: forall
             i_src0 i_tgt0 w0 (st_src0: st_local) (st_tgt0: st_local)
             fn varg rvs k_src k_tgt
             (K: forall vret,
-                paco8 _sim_itree bot8 _ _ RR true true w0 (st_src0, k_src vret) (st_tgt0, k_tgt vret)),
+                paco8 _sim_itree bot8 _ _ RR TT TT w0 (st_src0, k_src vret) (st_tgt0, k_tgt vret)),
             P i_src0 i_tgt0 w0 (st_src0, trigger (Syscall fn varg rvs) >>= k_src)
               (st_tgt0, trigger (Syscall fn varg rvs) >>= k_tgt))
         (INLINESRC: forall
@@ -321,75 +393,96 @@ Section SIM.
             f fn varg k_src i_tgt
             (FUN: alist_find fn fl_src = Some f)
             (* (IN: In (fn, f) fl_src) *)
-            (K: paco8 _sim_itree bot8 _ _ RR true i_tgt0 w0 (st_src, (f varg) >>= k_src) (st_tgt, i_tgt))
-            (IH: P true i_tgt0 w0 (st_src, (f varg) >>= k_src) (st_tgt, i_tgt)),
+            (K: paco8 _sim_itree bot8 _ _ RR TT i_tgt0 w0 (st_src, (f varg) >>= k_src) (st_tgt, i_tgt))
+            (IH: P TT i_tgt0 w0 (st_src, (f varg) >>= k_src) (st_tgt, i_tgt)),
             P i_src0 i_tgt0 w0 (st_src, trigger (Call fn varg) >>= k_src) (st_tgt, i_tgt))
         (INLINETGT: forall
             i_src0 i_tgt0 w0 st_src st_tgt
             f fn varg i_src k_tgt
             (FUN: alist_find fn fl_tgt = Some f)
             (* (IN: In (fn, f) fl_tgt) *)
-            (K: paco8 _sim_itree bot8 _ _ RR i_src0 true w0 (st_src, i_src) (st_tgt, (f varg) >>= k_tgt))
-            (IH: P i_src0 true w0 (st_src, i_src) (st_tgt, (f varg) >>= k_tgt)),
+            (K: paco8 _sim_itree bot8 _ _ RR i_src0 TT w0 (st_src, i_src) (st_tgt, (f varg) >>= k_tgt))
+            (IH: P i_src0 TT w0 (st_src, i_src) (st_tgt, (f varg) >>= k_tgt)),
             P i_src0 i_tgt0 w0 (st_src, i_src) (st_tgt, trigger (Call fn varg) >>= k_tgt))            
         (TAUSRC: forall
             i_src0 i_tgt0 w0 (st_src0: st_local) (st_tgt0: st_local)
             i_src i_tgt
-            (K: paco8 _sim_itree bot8 _ _ RR true i_tgt0 w0 (st_src0, i_src) (st_tgt0, i_tgt))
-            (IH: P true i_tgt0 w0 (st_src0, i_src) (st_tgt0, i_tgt)),
+            (K: paco8 _sim_itree bot8 _ _ RR TT i_tgt0 w0 (st_src0, i_src) (st_tgt0, i_tgt))
+            (IH: P TT i_tgt0 w0 (st_src0, i_src) (st_tgt0, i_tgt)),
             P i_src0 i_tgt0 w0 (st_src0, tau;; i_src) (st_tgt0, i_tgt))
         (TAUTGT: forall
             i_src0 i_tgt0 w0 (st_src0: st_local) (st_tgt0: st_local)
             i_src i_tgt
-            (K: paco8 _sim_itree bot8 _ _ RR i_src0 true w0 (st_src0, i_src) (st_tgt0, i_tgt))
-            (IH: P i_src0 true w0 (st_src0, i_src) (st_tgt0, i_tgt)),
+            (K: paco8 _sim_itree bot8 _ _ RR i_src0 TT w0 (st_src0, i_src) (st_tgt0, i_tgt))
+            (IH: P i_src0 TT w0 (st_src0, i_src) (st_tgt0, i_tgt)),
             P i_src0 i_tgt0 w0 (st_src0, i_src) (st_tgt0, tau;; i_tgt))            
         (CHOOSESRC: forall
             i_src0 i_tgt0 w0 (st_src0: st_local) (st_tgt0: st_local)
             X k_src i_tgt
-            (K: exists (x: X), <<SIM: paco8 _sim_itree bot8 _ _ RR true i_tgt0 w0 (st_src0, k_src x) (st_tgt0, i_tgt)>> /\ <<IH: P true i_tgt0 w0 (st_src0, k_src x) (st_tgt0, i_tgt)>>),
+            (K: exists (x: X), <<SIM: paco8 _sim_itree bot8 _ _ RR TT i_tgt0 w0 (st_src0, k_src x) (st_tgt0, i_tgt)>> /\ <<IH: P TT i_tgt0 w0 (st_src0, k_src x) (st_tgt0, i_tgt)>>),
             P i_src0 i_tgt0 w0 (st_src0, trigger (Choose X) >>= k_src)
               (st_tgt0, i_tgt))
         (CHOOSETGT: forall
             i_src0 i_tgt0 w0 (st_src0: st_local) (st_tgt0: st_local)
             X i_src k_tgt
-            (K: forall (x: X), <<SIMH: paco8 _sim_itree bot8 _ _ RR i_src0 true w0 (st_src0, i_src) (st_tgt0, k_tgt x)>> /\ <<IH: P i_src0 true w0 (st_src0, i_src) (st_tgt0, k_tgt x)>>),
+            (K: forall (x: X), <<SIMH: paco8 _sim_itree bot8 _ _ RR i_src0 TT w0 (st_src0, i_src) (st_tgt0, k_tgt x)>> /\ <<IH: P i_src0 TT w0 (st_src0, i_src) (st_tgt0, k_tgt x)>>),
             P i_src0 i_tgt0 w0 (st_src0, i_src)
               (st_tgt0, trigger (Choose X) >>= k_tgt))
         (TAKESRC: forall
             i_src0 i_tgt0 w0 (st_src0: st_local) (st_tgt0: st_local)
             X k_src i_tgt
-            (K: forall (x: X), <<SIM: paco8 _sim_itree bot8 _ _ RR true i_tgt0 w0 (st_src0, k_src x) (st_tgt0, i_tgt)>> /\ <<IH: P true i_tgt0 w0 (st_src0, k_src x) (st_tgt0, i_tgt)>>),
+            (K: forall (x: X), <<SIM: paco8 _sim_itree bot8 _ _ RR TT i_tgt0 w0 (st_src0, k_src x) (st_tgt0, i_tgt)>> /\ <<IH: P TT i_tgt0 w0 (st_src0, k_src x) (st_tgt0, i_tgt)>>),
             P i_src0 i_tgt0 w0 (st_src0, trigger (Take X) >>= k_src)
               (st_tgt0, i_tgt))
         (TAKETGT: forall
             i_src0 i_tgt0 w0 (st_src0: st_local) (st_tgt0: st_local)
             X i_src k_tgt
-            (K: exists (x: X), <<SIM:paco8 _sim_itree bot8 _ _ RR i_src0 true w0 (st_src0, i_src) (st_tgt0, k_tgt x)>> /\ <<IH: P i_src0 true w0 (st_src0, i_src) (st_tgt0, k_tgt x)>>),
+            (K: exists (x: X), <<SIM:paco8 _sim_itree bot8 _ _ RR i_src0 TT w0 (st_src0, i_src) (st_tgt0, k_tgt x)>> /\ <<IH: P i_src0 TT w0 (st_src0, i_src) (st_tgt0, k_tgt x)>>),
             P i_src0 i_tgt0 w0 (st_src0, i_src)
               (st_tgt0, trigger (Take X) >>= k_tgt))
         (SUPDATESRC: forall
             i_src0 i_tgt0 w0 (st_src0: st_local) (st_tgt0: st_local)
             X k_src i_tgt
             (run: st_local -> st_local * X )
-            (K: paco8 _sim_itree bot8 _ _ RR true i_tgt0 w0 (fst (run st_src0), k_src (snd (run st_src0))) (st_tgt0, i_tgt))
-            (IH: P true i_tgt0 w0 (fst (run st_src0), k_src (snd (run st_src0))) (st_tgt0, i_tgt)),
+            (K: paco8 _sim_itree bot8 _ _ RR TT i_tgt0 w0 (fst (run st_src0), k_src (snd (run st_src0))) (st_tgt0, i_tgt))
+            (IH: P TT i_tgt0 w0 (fst (run st_src0), k_src (snd (run st_src0))) (st_tgt0, i_tgt)),
             P i_src0 i_tgt0 w0 (st_src0, trigger (SUpdate run) >>= k_src) (st_tgt0, i_tgt))
         (SUPDATETGT: forall
             i_src0 i_tgt0 w0 (st_src0: st_local) (st_tgt0: st_local)
             X i_src k_tgt
             (run: st_local -> st_local * X )
-            (K: paco8 _sim_itree bot8 _ _ RR i_src0 true w0 (st_src0, i_src) (fst (run st_tgt0), k_tgt (snd (run st_tgt0))))
-            (IH:  P i_src0 true w0 (st_src0, i_src) (fst (run st_tgt0), k_tgt (snd (run st_tgt0)))),
-
-            P i_src0 i_tgt0 w0 (st_src0, i_src) (st_tgt0, trigger (SUpdate run) >>= k_tgt))       
+            (K: paco8 _sim_itree bot8 _ _ RR i_src0 TT w0 (st_src0, i_src) (fst (run st_tgt0), k_tgt (snd (run st_tgt0))))
+            (IH:  P i_src0 TT w0 (st_src0, i_src) (fst (run st_tgt0), k_tgt (snd (run st_tgt0)))),
+            P i_src0 i_tgt0 w0 (st_src0, i_src) (st_tgt0, trigger (SUpdate run) >>= k_tgt))      
+        (YIELDTGT: forall
+            i_src0 i_tgt0 w w0 st_src0 st_tgt0
+            k_src k_tgt
+            (WF: wf w0 (st_src0, st_tgt0))
+            (K: forall w1 st_tgt1 (WLE: le w0 w1) (WF: wf w1 (st_src0, st_tgt1)),
+                << SIMH: paco8 _sim_itree bot8 _ _ RR i_src0 YY w (st_src0, trigger Yield >>= k_src) (st_tgt1, k_tgt tt) >>
+                /\ << IH: P i_src0 YY w (st_src0, trigger Yield >>= k_src) (st_tgt1, k_tgt tt) >> ),
+            P i_src0 i_tgt0 w (st_src0, trigger Yield >>= k_src) (st_tgt0, trigger Yield >>= k_tgt))                
+        (YIELDSRC: forall
+            i_src0 i_tgt0 w0 st_src0 st_tgt0
+            k_src i_tgt
+            st_src1
+            (K: paco8 _sim_itree bot8 _ _ RR YY i_tgt0 w0 (st_src1, k_src tt) (st_tgt0, i_tgt))
+            (IH: P YY i_tgt0 w0 (st_src1, k_src tt) (st_tgt0, i_tgt)),
+            P i_src0 i_tgt0 w0 (st_src0, trigger Yield >>= k_src) (st_tgt0, i_tgt))
+        (SPAWN: forall
+            i_src0 i_tgt0 w w0 st_src0 st_tgt0
+            fn varg k_src k_tgt
+            (WF: wf w0 (st_src0, st_tgt0))
+            (K: forall w1 vret st_src1 st_tgt1 (WLE: le w0 w1) (WF: wf w1 (st_src1, st_tgt1)),
+                paco8 _sim_itree bot8 _ _ RR YY YY w (st_src1, k_src vret) (st_tgt1, k_tgt vret)),
+            P i_src0 i_tgt0 w (st_src0, trigger (Spawn fn varg) >>= k_src)
+              (st_tgt0, trigger (Spawn fn varg) >>= k_tgt))            
         (PROGRESS: forall
-            i_src0 i_tgt0 w0 (st_src0: st_local) (st_tgt0: st_local)
+            i_flag w0 (st_src0: st_local) (st_tgt0: st_local)
             i_src i_tgt
-            (SIM: paco8 _sim_itree bot8 _ _ RR false false w0 (st_src0, i_src) (st_tgt0, i_tgt))
-            (SRC: i_src0 = true)
-            (TGT: i_tgt0 = true),
-            P true true w0 (st_src0, i_src) (st_tgt0, i_tgt))
+            (SIM: paco8 _sim_itree bot8 _ _ RR BB BB w0 (st_src0, i_src) (st_tgt0, i_tgt))
+            (FLAG: i_flag = TT \/ i_flag = YY),
+            P i_flag i_flag w0 (st_src0, i_src) (st_tgt0, i_tgt))
     :
       forall i_src0 i_tgt0 w0 st_src st_tgt
              (SIM: paco8 _sim_itree bot8 _ _ RR i_src0 i_tgt0 w0 st_src st_tgt),
@@ -411,13 +504,16 @@ Section SIM.
     { eapply TAKETGT; eauto. des. esplits; eauto. }
     { eapply SUPDATESRC; eauto. }
     { eapply SUPDATETGT; eauto. }
+    { eapply YIELDTGT; et. i. exploit K; et. i. des. esplits; et. }
+    { eapply YIELDSRC; eauto. }
+    { eapply SPAWN; et. i. exploit K; et. i. pclearbot. et. }
     { eapply PROGRESS; eauto. pclearbot. auto. }
 
   Qed.
 
-  Variant sim_itree_indC (sim_itree: forall (R_src R_tgt: Type) (RR: st_local -> st_local -> R_src -> R_tgt -> Prop), bool -> bool -> world -> st_local * itree Es R_src -> st_local * itree Es R_tgt -> Prop)
+  Variant sim_itree_indC (sim_itree: forall (R_src R_tgt: Type) (RR: st_local -> st_local -> R_src -> R_tgt -> Prop), flag -> flag -> world -> st_local * itree Es R_src -> st_local * itree Es R_tgt -> Prop)
           {R_src R_tgt} (RR: st_local -> st_local -> R_src -> R_tgt -> Prop)
-    : bool -> bool -> world -> st_local * itree Es R_src -> st_local * itree Es R_tgt -> Prop :=
+    : flag -> flag -> world -> st_local * itree Es R_src -> st_local * itree Es R_tgt -> Prop :=
   | sim_itree_indC_ret
       i_src0 i_tgt0 w0 st_src0 st_tgt0
       v_src v_tgt
@@ -429,7 +525,7 @@ Section SIM.
       fn varg k_src k_tgt
       (WF: wf w0 (st_src0, st_tgt0))
       (K: forall w1 vret st_src1 st_tgt1 (WLE: le w0 w1) (WF: wf w1 (st_src1, st_tgt1)),
-          sim_itree _ _ RR true true w (st_src1, k_src vret) (st_tgt1, k_tgt vret))
+          sim_itree _ _ RR TT TT w (st_src1, k_src vret) (st_tgt1, k_tgt vret))
     :
       sim_itree_indC  sim_itree RR i_src0 i_tgt0 w (st_src0, trigger (Call fn varg) >>= k_src)
                      (st_tgt0, trigger (Call fn varg) >>= k_tgt)
@@ -437,7 +533,7 @@ Section SIM.
       i_src0 i_tgt0 w0 (st_src0: st_local) (st_tgt0: st_local)
       fn varg rvs k_src k_tgt
       (K: forall vret,
-          sim_itree _ _ RR true true w0 (st_src0, k_src vret) (st_tgt0, k_tgt vret))
+          sim_itree _ _ RR TT TT w0 (st_src0, k_src vret) (st_tgt0, k_tgt vret))
     :
       sim_itree_indC  sim_itree RR i_src0 i_tgt0 w0 (st_src0, trigger (Syscall fn varg rvs) >>= k_src)
                      (st_tgt0, trigger (Syscall fn varg rvs) >>= k_tgt)
@@ -447,7 +543,7 @@ Section SIM.
       f fn varg k_src i_tgt
       (FUN: alist_find fn fl_src = Some f)
       (* (IN: In (fn, f) fl_src) *)
-      (K: sim_itree _ _ RR true i_tgt0 w0 (st_src0, (f varg) >>= k_src) (st_tgt0, i_tgt))
+      (K: sim_itree _ _ RR TT i_tgt0 w0 (st_src0, (f varg) >>= k_src) (st_tgt0, i_tgt))
     :
       sim_itree_indC  sim_itree RR i_src0 i_tgt0 w0 (st_src0, trigger (Call fn varg) >>= k_src) (st_tgt0, i_tgt)
 
@@ -456,35 +552,35 @@ Section SIM.
       f fn varg i_src k_tgt
       (FUN: alist_find fn fl_tgt = Some f)
       (* (IN: In (fn, f) fl_tgt) *)
-      (K: sim_itree _ _ RR i_src0 true w0 (st_src0, i_src) (st_tgt0, (f varg) >>= k_tgt))
+      (K: sim_itree _ _ RR i_src0 TT w0 (st_src0, i_src) (st_tgt0, (f varg) >>= k_tgt))
     :
       sim_itree_indC  sim_itree RR i_src0 i_tgt0 w0 (st_src0, i_src) (st_tgt0, trigger (Call fn varg) >>= k_tgt)
  
   | sim_itree_indC_tau_src
       i_src0 i_tgt0 w0 (st_src0: st_local) (st_tgt0: st_local)
       i_src i_tgt
-      (K: sim_itree _ _ RR true i_tgt0 w0 (st_src0, i_src) (st_tgt0, i_tgt))
+      (K: sim_itree _ _ RR TT i_tgt0 w0 (st_src0, i_src) (st_tgt0, i_tgt))
     :
       sim_itree_indC  sim_itree RR i_src0 i_tgt0 w0 (st_src0, tau;; i_src) (st_tgt0, i_tgt)
 
   | sim_itree_indC_tau_tgt
       i_src0 i_tgt0 w0 (st_src0: st_local) (st_tgt0: st_local)
       i_src i_tgt
-      (K: sim_itree _ _ RR i_src0 true w0 (st_src0, i_src) (st_tgt0, i_tgt))
+      (K: sim_itree _ _ RR i_src0 TT w0 (st_src0, i_src) (st_tgt0, i_tgt))
     :
       sim_itree_indC  sim_itree RR i_src0 i_tgt0 w0 (st_src0, i_src) (st_tgt0, tau;; i_tgt)
 
   | sim_itree_indC_choose_src
       i_src0 i_tgt0 w0 (st_src0: st_local) (st_tgt0: st_local)
       X k_src i_tgt
-      (K: exists (x: X), sim_itree _ _ RR true i_tgt0 w0 (st_src0, k_src x) (st_tgt0, i_tgt))
+      (K: exists (x: X), sim_itree _ _ RR TT i_tgt0 w0 (st_src0, k_src x) (st_tgt0, i_tgt))
     :
       sim_itree_indC  sim_itree RR i_src0 i_tgt0 w0 (st_src0, trigger (Choose X) >>= k_src)
                      (st_tgt0, i_tgt)
   | sim_itree_indC_choose_tgt
       i_src0 i_tgt0 w0 (st_src0: st_local) (st_tgt0: st_local)
       X i_src k_tgt
-      (K: forall (x: X), sim_itree _ _ RR i_src0 true w0 (st_src0, i_src) (st_tgt0, k_tgt x))
+      (K: forall (x: X), sim_itree _ _ RR i_src0 TT w0 (st_src0, i_src) (st_tgt0, k_tgt x))
     :
       sim_itree_indC  sim_itree RR i_src0 i_tgt0 w0 (st_src0, i_src)
                      (st_tgt0, trigger (Choose X) >>= k_tgt)
@@ -492,14 +588,14 @@ Section SIM.
   | sim_itree_indC_take_src
       i_src0 i_tgt0 w0 (st_src0: st_local) (st_tgt0: st_local)
       X k_src i_tgt
-      (K: forall (x: X), sim_itree _ _ RR true i_tgt0 w0 (st_src0, k_src x) (st_tgt0, i_tgt))
+      (K: forall (x: X), sim_itree _ _ RR TT i_tgt0 w0 (st_src0, k_src x) (st_tgt0, i_tgt))
     :
       sim_itree_indC  sim_itree RR i_src0 i_tgt0 w0 (st_src0, trigger (Take X) >>= k_src)
                      (st_tgt0, i_tgt)
   | sim_itree_indC_take_tgt
       i_src0 i_tgt0 w0 (st_src0: st_local) (st_tgt0: st_local)
       X i_src k_tgt
-      (K: exists (x: X), sim_itree _ _ RR i_src0 true w0 (st_src0, i_src) (st_tgt0, k_tgt x))
+      (K: exists (x: X), sim_itree _ _ RR i_src0 TT w0 (st_src0, i_src) (st_tgt0, k_tgt x))
     :
       sim_itree_indC  sim_itree RR i_src0 i_tgt0 w0 (st_src0, i_src)
                      (st_tgt0, trigger (Take X) >>= k_tgt)
@@ -508,7 +604,7 @@ Section SIM.
       i_src0 i_tgt0 w0 (st_src0: st_local) (st_tgt0: st_local)
       X k_src i_tgt
       (run: st_local -> st_local * X )
-      (K: sim_itree _ _ RR true i_tgt0 w0 (fst (run st_src0), k_src (snd (run st_src0))) (st_tgt0, i_tgt))
+      (K: sim_itree _ _ RR TT i_tgt0 w0 (fst (run st_src0), k_src (snd (run st_src0))) (st_tgt0, i_tgt))
     :
       sim_itree_indC  sim_itree RR i_src0 i_tgt0 w0 (st_src0, trigger (SUpdate run) >>= k_src) (st_tgt0, i_tgt)
 
@@ -516,10 +612,38 @@ Section SIM.
       i_src0 i_tgt0 w0 (st_src0: st_local) (st_tgt0: st_local)
       X i_src k_tgt
       (run: st_local -> st_local * X )
-      (K: sim_itree _ _ RR i_src0 true w0 (st_src0, i_src) (fst (run st_tgt0), k_tgt (snd (run st_tgt0))))
+      (K: sim_itree _ _ RR i_src0 TT w0 (st_src0, i_src) (fst (run st_tgt0), k_tgt (snd (run st_tgt0))))
     :
       sim_itree_indC  sim_itree RR i_src0 i_tgt0 w0 (st_src0, i_src) (st_tgt0, trigger (SUpdate run) >>= k_tgt)
-  .
+
+  | sim_itree_indC_yield_tgt
+      i_src0 i_tgt0 w w0 st_src0 st_tgt0
+      k_src k_tgt
+      (WF: wf w0 (st_src0, st_tgt0))
+      (K: forall w1 st_tgt1 (WLE: le w0 w1) (WF: wf w1 (st_src0, st_tgt1)),
+        sim_itree _ _ RR i_src0 YY w (st_src0, trigger Yield >>= k_src) (st_tgt1, k_tgt tt))
+    :
+      sim_itree_indC sim_itree RR i_src0 i_tgt0 w (st_src0, trigger Yield >>= k_src) (st_tgt0, trigger Yield >>= k_tgt)
+ 
+  | sim_itree_indC_yield_src
+      i_src0 i_tgt0 w0 st_src0 st_tgt0
+      k_src i_tgt
+      st_src1
+      (K: sim_itree _ _ RR YY i_tgt0 w0 (st_src1, k_src tt) (st_tgt0, i_tgt))
+    :
+      sim_itree_indC sim_itree RR i_src0 i_tgt0 w0 (st_src0, trigger Yield >>= k_src) (st_tgt0, i_tgt)
+
+  | sim_itree_indC_spawn
+      i_src0 i_tgt0 w w0 st_src0 st_tgt0
+      fn varg k_src k_tgt
+      (WF: wf w0 (st_src0, st_tgt0))
+      (K: forall w1 vret st_src1 st_tgt1 (WLE: le w0 w1) (WF: wf w1 (st_src1, st_tgt1)),
+          sim_itree _ _ RR YY YY w (st_src1, k_src vret) (st_tgt1, k_tgt vret))
+    :
+      sim_itree_indC  sim_itree RR i_src0 i_tgt0 w (st_src0, trigger (Spawn fn varg) >>= k_src)
+                     (st_tgt0, trigger (Spawn fn varg) >>= k_tgt)                    
+
+      .
 
   Lemma sim_itree_indC_mon: monotone8 sim_itree_indC.
   Proof.
@@ -546,11 +670,14 @@ Section SIM.
     { econs 11; eauto. des. esplits; eauto. eapply sim_itree_mon; eauto. i. eapply rclo8_base. eauto. }
     { econs 12; eauto. des. esplits; eauto. eapply sim_itree_mon; eauto. i. eapply rclo8_base. eauto.  }
     { econs 13; eauto. des. esplits; eauto.  eapply sim_itree_mon; eauto. i. eapply rclo8_base. eauto.  }
+    { econs 14; eauto. i. eapply sim_itree_mon; eauto. i. eapply rclo8_base. eauto. }
+    { econs 15; eauto. eapply sim_itree_mon; eauto. i. eapply rclo8_base. eauto. }
+    { econs 16; et. i. exploit K; et. i. eapply rclo8_base. et. }
   Qed.
 
-  Variant sim_itreeC (r g: forall (R_src R_tgt: Type) (RR: st_local -> st_local -> R_src -> R_tgt -> Prop), bool -> bool -> world -> st_local * itree Es R_src -> st_local * itree Es R_tgt -> Prop)
+  Variant sim_itreeC (r g: forall (R_src R_tgt: Type) (RR: st_local -> st_local -> R_src -> R_tgt -> Prop), flag -> flag -> world -> st_local * itree Es R_src -> st_local * itree Es R_tgt -> Prop)
           {R_src R_tgt} (RR: st_local -> st_local -> R_src -> R_tgt -> Prop)
-    : bool -> bool -> world -> st_local * itree Es R_src -> st_local * itree Es R_tgt -> Prop :=
+    : flag -> flag -> world -> st_local * itree Es R_src -> st_local * itree Es R_tgt -> Prop :=
   | sim_itreeC_ret
       i_src0 i_tgt0 w0 st_src0 st_tgt0
       v_src v_tgt
@@ -562,7 +689,7 @@ Section SIM.
       fn varg k_src k_tgt
       (WF: wf w0 (st_src0, st_tgt0))
       (K: forall w1 vret st_src1 st_tgt1 (WLE: le w0 w1) (WF: wf w1 (st_src1, st_tgt1)),
-          g _ _ RR true true w (st_src1, k_src vret) (st_tgt1, k_tgt vret))
+          g _ _ RR TT TT w (st_src1, k_src vret) (st_tgt1, k_tgt vret))
     :
       sim_itreeC r g RR i_src0 i_tgt0 w (st_src0, trigger (Call fn varg) >>= k_src)
                  (st_tgt0, trigger (Call fn varg) >>= k_tgt)
@@ -570,7 +697,7 @@ Section SIM.
       i_src0 i_tgt0 w0 (st_src0: st_local) (st_tgt0: st_local)
       fn varg rvs k_src k_tgt
       (K: forall vret,
-          g _ _ RR true true w0 (st_src0, k_src vret) (st_tgt0, k_tgt vret))
+          g _ _ RR TT TT w0 (st_src0, k_src vret) (st_tgt0, k_tgt vret))
     :
       sim_itreeC r g RR i_src0 i_tgt0 w0 (st_src0, trigger (Syscall fn varg rvs) >>= k_src)
                  (st_tgt0, trigger (Syscall fn varg rvs) >>= k_tgt)
@@ -580,7 +707,7 @@ Section SIM.
       f fn varg k_src i_tgt
       (FUN: alist_find fn fl_src = Some f)
       (* (IN: In (fn, f) fl_src) *)
-      (K: r _ _ RR true i_tgt0 w0 (st_src0, (f varg) >>= k_src) (st_tgt0, i_tgt))
+      (K: r _ _ RR TT i_tgt0 w0 (st_src0, (f varg) >>= k_src) (st_tgt0, i_tgt))
     :
       sim_itreeC r g RR i_src0 i_tgt0 w0 (st_src0, trigger (Call fn varg) >>= k_src) (st_tgt0, i_tgt)
 
@@ -589,21 +716,21 @@ Section SIM.
       f fn varg i_src k_tgt
       (FUN: alist_find fn fl_tgt = Some f)
       (* (IN: In (fn, f) fl_tgt) *)
-      (K: r _ _ RR i_src0 true w0 (st_src0, i_src) (st_tgt0, (f varg) >>= k_tgt))
+      (K: r _ _ RR i_src0 TT w0 (st_src0, i_src) (st_tgt0, (f varg) >>= k_tgt))
     :
       sim_itreeC r g RR i_src0 i_tgt0 w0 (st_src0, i_src) (st_tgt0, trigger (Call fn varg) >>= k_tgt)
 
   | sim_itreeC_tau_src
       i_src0 i_tgt0 w0 (st_src0: st_local) (st_tgt0: st_local)
       i_src i_tgt
-      (K: r _ _ RR true i_tgt0 w0 (st_src0, i_src) (st_tgt0, i_tgt))
+      (K: r _ _ RR TT i_tgt0 w0 (st_src0, i_src) (st_tgt0, i_tgt))
     :
       sim_itreeC r g RR i_src0 i_tgt0 w0 (st_src0, tau;; i_src) (st_tgt0, i_tgt)
 
   | sim_itreeC_tau_tgt
       i_src0 i_tgt0 w0 (st_src0: st_local) (st_tgt0: st_local)
       i_src i_tgt
-      (K: r _ _ RR i_src0 true w0 (st_src0, i_src) (st_tgt0, i_tgt))
+      (K: r _ _ RR i_src0 TT w0 (st_src0, i_src) (st_tgt0, i_tgt))
     :
       sim_itreeC r g RR i_src0 i_tgt0 w0 (st_src0, i_src) (st_tgt0, tau;; i_tgt)
 
@@ -611,28 +738,28 @@ Section SIM.
   | sim_itreeC_choose_src
       i_src0 i_tgt0 w0 (st_src0: st_local) (st_tgt0: st_local)
       X k_src i_tgt
-      (K: exists (x: X), r _ _ RR true i_tgt0 w0 (st_src0, k_src x) (st_tgt0, i_tgt))
+      (K: exists (x: X), r _ _ RR TT i_tgt0 w0 (st_src0, k_src x) (st_tgt0, i_tgt))
     :
       sim_itreeC r g RR i_src0 i_tgt0 w0 (st_src0, trigger (Choose X) >>= k_src)
                  (st_tgt0, i_tgt)
   | sim_itreeC_choose_tgt
       i_src0 i_tgt0 w0 (st_src0: st_local) (st_tgt0: st_local)
       X i_src k_tgt
-      (K: forall (x: X), r _ _ RR i_src0 true w0 (st_src0, i_src) (st_tgt0, k_tgt x))
+      (K: forall (x: X), r _ _ RR i_src0 TT w0 (st_src0, i_src) (st_tgt0, k_tgt x))
     :
       sim_itreeC r g RR i_src0 i_tgt0 w0 (st_src0, i_src)
                  (st_tgt0, trigger (Choose X) >>= k_tgt)
   | sim_itreeC_take_src
       i_src0 i_tgt0 w0 (st_src0: st_local) (st_tgt0: st_local)
       X k_src i_tgt
-      (K: forall (x: X), r _ _ RR true i_tgt0 w0 (st_src0, k_src x) (st_tgt0, i_tgt))
+      (K: forall (x: X), r _ _ RR TT i_tgt0 w0 (st_src0, k_src x) (st_tgt0, i_tgt))
     :
       sim_itreeC r g RR i_src0 i_tgt0 w0 (st_src0, trigger (Take X) >>= k_src)
                  (st_tgt0, i_tgt)
   | sim_itreeC_take_tgt
       i_src0 i_tgt0 w0 (st_src0: st_local) (st_tgt0: st_local)
       X i_src k_tgt
-      (K: exists (x: X), r _ _ RR i_src0 true w0 (st_src0, i_src) (st_tgt0, k_tgt x))
+      (K: exists (x: X), r _ _ RR i_src0 TT w0 (st_src0, i_src) (st_tgt0, k_tgt x))
     :
       sim_itreeC r g RR i_src0 i_tgt0 w0 (st_src0, i_src)
                  (st_tgt0, trigger (Take X) >>= k_tgt)
@@ -640,7 +767,7 @@ Section SIM.
       i_src0 i_tgt0 w0 (st_src0: st_local) (st_tgt0: st_local)
       X k_src i_tgt
       (run: st_local -> st_local * X )
-      (K: r _ _ RR true i_tgt0 w0 (fst (run st_src0), k_src (snd (run st_src0))) (st_tgt0, i_tgt))
+      (K: r _ _ RR TT i_tgt0 w0 (fst (run st_src0), k_src (snd (run st_src0))) (st_tgt0, i_tgt))
     :
       sim_itreeC r g RR i_src0 i_tgt0 w0 (st_src0, trigger (SUpdate run) >>= k_src) (st_tgt0, i_tgt)
 
@@ -648,10 +775,34 @@ Section SIM.
       i_src0 i_tgt0 w0 (st_src0: st_local) (st_tgt0: st_local)
       X i_src k_tgt
       (run: st_local -> st_local * X )
-      (K: r _ _ RR i_src0 true w0 (st_src0, i_src) (fst (run st_tgt0), k_tgt (snd (run st_tgt0))))
+      (K: r _ _ RR i_src0 TT w0 (st_src0, i_src) (fst (run st_tgt0), k_tgt (snd (run st_tgt0))))
     :
       sim_itreeC r g RR i_src0 i_tgt0 w0 (st_src0, i_src) (st_tgt0, trigger (SUpdate run) >>= k_tgt)
 
+  | sim_itreeC_yield_tgt
+      i_src0 i_tgt0 w w0 st_src0 st_tgt0
+      k_src k_tgt
+      (WF: wf w0 (st_src0, st_tgt0))
+      (K: forall w1 st_tgt1 (WLE: le w0 w1) (WF: wf w1 (st_src0, st_tgt1)),
+        r _ _ RR i_src0 YY w (st_src0, trigger Yield >>= k_src) (st_tgt1, k_tgt tt))
+    :
+      sim_itreeC r g RR i_src0 i_tgt0 w (st_src0, trigger Yield >>= k_src) (st_tgt0, trigger Yield >>= k_tgt)
+  | sim_itreeC_yield_src
+      i_src0 i_tgt0 w0 st_src0 st_tgt0
+      k_src i_tgt
+      st_src1
+      (K: r _ _ RR YY i_tgt0 w0 (st_src1, k_src tt) (st_tgt0, i_tgt))
+    :
+      sim_itreeC r g RR i_src0 i_tgt0 w0 (st_src0, trigger Yield >>= k_src) (st_tgt0, i_tgt)
+  | sim_itreeC_spawn
+      i_src0 i_tgt0 w w0 st_src0 st_tgt0
+      fn varg k_src k_tgt
+      (WF: wf w0 (st_src0, st_tgt0))
+      (K: forall w1 vret st_src1 st_tgt1 (WLE: le w0 w1) (WF: wf w1 (st_src1, st_tgt1)),
+          g _ _ RR YY YY w (st_src1, k_src vret) (st_tgt1, k_tgt vret))
+    :
+      sim_itreeC r g RR i_src0 i_tgt0 w (st_src0, trigger (Spawn fn varg) >>= k_src)
+                 (st_tgt0, trigger (Spawn fn varg) >>= k_tgt) 
   .
 
   Lemma sim_itreeC_spec_aux:
@@ -671,6 +822,9 @@ Section SIM.
     { guclo sim_itree_indC_spec. econs 11; eauto. des. esplits; eauto. gbase. eauto. }
     { guclo sim_itree_indC_spec. econs 12; eauto. gbase. eauto. }
     { guclo sim_itree_indC_spec. econs 13; eauto.  gbase. eauto. }
+    { guclo sim_itree_indC_spec. econs 14; eauto. i. gbase. eauto. }
+    { guclo sim_itree_indC_spec. econs 15; eauto. gbase. eauto. }
+    { gstep. econs 16; et. i. gbase. et. }
   Qed.
 
   Lemma sim_itreeC_spec r g
@@ -686,22 +840,31 @@ Section SIM.
     { i. eapply gupaco8_mon; eauto. }
   Qed.
 
-  Lemma sim_itree_progress_flag R0 R1 RR w r g st_src0 st_tgt0
-        (SIM: gpaco8 _sim_itree (cpn8 _sim_itree) g g R0 R1 RR false false w st_src0 st_tgt0)
+  Lemma sim_itree_progress_flag R0 R1 RR w f r g st_src0 st_tgt0
+        (SIM: gpaco8 _sim_itree (cpn8 _sim_itree) g g R0 R1 RR BB BB w st_src0 st_tgt0)
+        (FLAG: f = TT \/ f = YY)
     :
-      gpaco8 _sim_itree (cpn8 _sim_itree) r g R0 R1 RR true true w st_src0 st_tgt0.
+      gpaco8 _sim_itree (cpn8 _sim_itree) r g R0 R1 RR f f w st_src0 st_tgt0.
+  Proof.
+    gstep. destruct st_src0, st_tgt0. des; clarify; et.
+  Qed.
+(* 
+  Lemma sim_itree_progress_y_flag R0 R1 RR w r g st_src0 st_tgt0
+        (SIM: gpaco8 _sim_itree (cpn8 _sim_itree) g g R0 R1 RR BB BB w st_src0 st_tgt0)
+    :
+      gpaco8 _sim_itree (cpn8 _sim_itree) r g R0 R1 RR YY YY w st_src0 st_tgt0.
   Proof.
     gstep. destruct st_src0, st_tgt0. econs; eauto. 
-  Qed.
+  Qed.   *)
 
   Lemma sim_itree_flag_mon
         (sim_itree: forall (R_src R_tgt: Type)
-                           (RR: st_local -> st_local -> R_src -> R_tgt -> Prop), bool -> bool -> world -> st_local * itree Es R_src -> st_local * itree Es R_tgt -> Prop)
+                           (RR: st_local -> st_local -> R_src -> R_tgt -> Prop), flag -> flag -> world -> st_local * itree Es R_src -> st_local * itree Es R_tgt -> Prop)
         R_src R_tgt (RR: st_local -> st_local -> R_src -> R_tgt -> Prop)
         f_src0 f_tgt0 f_src1 f_tgt1 w st_src0 st_tgt0
         (SIM: @_sim_itree sim_itree _ _ RR f_src0 f_tgt0 w st_src0 st_tgt0)
-        (SRC: f_src0 = true -> f_src1 = true)
-        (TGT: f_tgt0 = true -> f_tgt1 = true)
+        (SRC: (f_src0 = TT -> f_src1 = TT) /\ (f_src0 = YY -> f_src1 = YY))
+        (TGT: (f_tgt0 = TT -> f_tgt1 = TT) /\ (f_tgt0 = YY -> f_tgt1 = YY))
     :
       @_sim_itree sim_itree _ _ RR f_src1 f_tgt1 w st_src0 st_tgt0.
   Proof.
@@ -719,28 +882,34 @@ Section SIM.
     { econs 10; eauto. i. exploit K; eauto. i. des. eauto. }
     { econs 11; eauto. des. esplits; eauto. }
     { econs 12; eauto. }
-    { econs 13; eauto. } 
-    { exploit SRC0; auto. exploit TGT0; auto. i. clarify. econs; eauto. }
+    { econs 13; eauto. }
+    { econs 14; eauto. i. exploit K; et. i. des. et. }
+    { econs 15; eauto. }
+    { econs 16; et. }
+    { des.
+      { exploit SRC; et. exploit TGT; et. i. clarify. econs; et.   }
+      { exploit SRC0; et. exploit TGT0; et. i. clarify. econs; et. }
+    }
   Qed.
 
 
   Definition sim_fsem: relation (Any.t -> itree Es Any.t) :=
     (eq ==> (fun it_src it_tgt => forall w mrs_src mrs_tgt (SIMMRS: wf w (mrs_src, mrs_tgt)),
-                 sim_itree false false w (mrs_src, it_src)
+                 sim_itree BB BB w (mrs_src, it_src)
                            (mrs_tgt, it_tgt)))%signature
   .
 
   Definition sim_fnsem: relation (string * (Any.t -> itree Es Any.t)) := RelProd eq sim_fsem.
 
   Variant lflagC (r: forall (R_src R_tgt: Type)
-    (RR: st_local -> st_local -> R_src -> R_tgt -> Prop), bool -> bool -> world -> st_local * itree Es R_src -> st_local * itree Es R_tgt -> Prop)
+    (RR: st_local -> st_local -> R_src -> R_tgt -> Prop), flag -> flag -> world -> st_local * itree Es R_src -> st_local * itree Es R_tgt -> Prop)
           {R_src R_tgt} (RR: st_local -> st_local -> R_src -> R_tgt -> Prop)
-    : bool -> bool -> world -> st_local * itree Es R_src -> st_local * itree Es R_tgt -> Prop :=
+    : flag -> flag -> world -> st_local * itree Es R_src -> st_local * itree Es R_tgt -> Prop :=
   | lflagC_intro
       f_src0 f_src1 f_tgt0 f_tgt1 w st_src st_tgt
       (SIM: r _ _ RR f_src0 f_tgt0 w st_src st_tgt)
-      (SRC: f_src0 = true -> f_src1 = true)
-      (TGT: f_tgt0 = true -> f_tgt1 = true)
+      (SRC: (f_src0 = TT -> f_src1 = TT) /\ (f_src0 = YY -> f_src1 = YY))
+      (TGT: (f_tgt0 = TT -> f_tgt1 = TT) /\ (f_tgt0 = YY -> f_tgt1 = YY))
     :
       lflagC r RR f_src1 f_tgt1 w st_src st_tgt
   .
@@ -775,34 +944,40 @@ Section SIM.
     { econs 11; eauto. des. esplits; eauto. }
     { econs 12; eauto. }
     { econs 13; eauto. }
-    { exploit SRC0; auto. exploit TGT0; auto. i. clarify. econs 14; eauto.
-      eapply rclo8_base; auto. }
+    { econs 14; et. i. exploit K; et. i. des. et. }
+    { econs 15; et. }
+    { econs 16; et. i. exploit K; et. i. des. eapply rclo8_base; et.  }
+    { des.
+      { exploit SRC; et. exploit TGT; et. i. clarify. econs; et. eapply rclo8_base; et. }
+      { exploit SRC0; et. exploit TGT0; et. i. clarify. econs; et. eapply rclo8_base; et. }
+    }      
   Qed.
 
   Lemma sim_itree_flag_down  R0 R1 RR r g w st_src0 st_tgt0 f_src f_tgt
-        (SIM: gpaco8 _sim_itree (cpn8 _sim_itree) r g R0 R1 RR false false w st_src0 st_tgt0)
+        (SIM: gpaco8 _sim_itree (cpn8 _sim_itree) r g R0 R1 RR BB BB w st_src0 st_tgt0)
     :
       gpaco8 _sim_itree (cpn8 _sim_itree) r g R0 R1 RR f_src f_tgt w st_src0 st_tgt0.
   Proof.
-    guclo lflagC_spec. econs; eauto.
+    guclo lflagC_spec. econs; eauto; clarify.
   Qed.
 
-  Lemma sim_itree_bot_flag_up  R0 R1 RR w st_src0 st_tgt0 f_src f_tgt
-        (SIM: paco8 _sim_itree bot8 R0 R1 RR true true w st_src0 st_tgt0)
+  Lemma sim_itree_bot_flag_up  R0 R1 RR w st_src0 st_tgt0 f f_src f_tgt
+        (SIM: paco8 _sim_itree bot8 R0 R1 RR f f w st_src0 st_tgt0)
+        (FLAG: f = TT \/ f = YY )
     :
       paco8 _sim_itree bot8 R0 R1 RR f_src f_tgt w st_src0 st_tgt0.
   Proof.
-    ginit. remember true in SIM at 1. remember true in SIM at 1.
-    clear Heqb Heqb0. revert w st_src0 st_tgt0 f_src f_tgt b b0 SIM.
+    ginit. remember f in SIM at 1. remember f in SIM at 1.
+    clear Heqf0 Heqf1. revert w st_src0 st_tgt0 f_src f_tgt f0 f1 SIM.
     gcofix CIH. 
     i. revert f_src f_tgt.
 
     (* TODO: why induction using sim_itree_ind doesn't work? *)
-    pattern b, b0, w, st_src0, st_tgt0.
+    pattern f0, f1, w, st_src0, st_tgt0.
     match goal with
-    | |- ?P b b0 w st_src0 st_tgt0 => set P
+    | |- ?P f0 f1 w st_src0 st_tgt0 => set P
     end.
-    revert b b0 w st_src0 st_tgt0 SIM.
+    revert f0 f1 w st_src0 st_tgt0 SIM.
     eapply (@sim_itree_ind R0 R1 RR P); subst P; ss; i; clarify.
     { guclo sim_itree_indC_spec. econs 1; eauto. }
     { gstep. econs 2; eauto. i. gbase. eapply CIH; eauto. }
@@ -811,19 +986,22 @@ Section SIM.
     { guclo sim_itree_indC_spec. econs 5; eauto. } 
     { guclo sim_itree_indC_spec. econs 6; eauto. } 
     { guclo sim_itree_indC_spec. econs 7; eauto. } 
-    { guclo sim_itree_indC_spec. econs 8; eauto. des. esplits; eauto. }
-    { guclo sim_itree_indC_spec. econs 9; eauto. i. hexploit K; eauto. i. des. esplits; eauto. }
-    { guclo sim_itree_indC_spec. econs 10; eauto. i. hexploit K; eauto. i. des. esplits; eauto. }
-    { guclo sim_itree_indC_spec. econs 11; eauto. des. esplits; eauto. }
+    { guclo sim_itree_indC_spec. econs 8; eauto. des; et. }
+    { guclo sim_itree_indC_spec. econs 9; eauto. i. hexploit K; eauto. i. des; esplits; eauto. }
+    { guclo sim_itree_indC_spec. econs 10; eauto. i. hexploit K; eauto. i. des; esplits; eauto. }
+    { guclo sim_itree_indC_spec. econs 11; eauto. des; esplits; eauto. }
     { guclo sim_itree_indC_spec. econs 12; eauto. } 
-    { guclo sim_itree_indC_spec. econs 13; eauto. } 
+    { guclo sim_itree_indC_spec. econs 13; eauto. }
+    { guclo sim_itree_indC_spec. econs 14; et. i. hexploit K; et. i. des; esplits; et. } 
+    { guclo sim_itree_indC_spec. econs 15; et. }
+    { gstep. econs 16; et. i. gbase. eapply CIH; et. }
     { eapply sim_itree_flag_down. gfinal. right.
       eapply paco8_mon; eauto. ss.
     }
   Qed.
 
-  Variant lbindR (r s: forall S_src S_tgt (SS: st_local -> st_local -> S_src -> S_tgt -> Prop), bool -> bool -> world -> st_local * itree Es S_src -> st_local * itree Es S_tgt -> Prop):
-    forall S_src S_tgt (SS: st_local -> st_local -> S_src -> S_tgt -> Prop), bool -> bool -> world -> st_local * itree Es S_src -> st_local * itree Es S_tgt -> Prop :=
+  Variant lbindR (r s: forall S_src S_tgt (SS: st_local -> st_local -> S_src -> S_tgt -> Prop), flag -> flag -> world -> st_local * itree Es S_src -> st_local * itree Es S_tgt -> Prop):
+    forall S_src S_tgt (SS: st_local -> st_local -> S_src -> S_tgt -> Prop), flag -> flag -> world -> st_local * itree Es S_src -> st_local * itree Es S_tgt -> Prop :=
   | lbindR_intro
       f_src f_tgt w0 w1
       R_src R_tgt RR
@@ -833,7 +1011,7 @@ Section SIM.
 
       S_src S_tgt SS
       (k_src: ktree Es R_src S_src) (k_tgt: ktree Es R_tgt S_tgt)
-      (SIMK: forall st_src1 st_tgt1 vret_src vret_tgt (SIM: RR st_src1 st_tgt1 vret_src vret_tgt), s _ _ SS false false w1 (st_src1, k_src vret_src) (st_tgt1, k_tgt vret_tgt))
+      (SIMK: forall st_src1 st_tgt1 vret_src vret_tgt (SIM: RR st_src1 st_tgt1 vret_src vret_tgt), s _ _ SS BB BB w1 (st_src1, k_src vret_src) (st_tgt1, k_tgt vret_tgt))
     :
       lbindR r s SS f_src f_tgt w1 (st_src0, ITree.bind i_src k_src) (st_tgt0, ITree.bind i_tgt k_tgt)
   .
@@ -878,8 +1056,14 @@ Section SIM.
     + rewrite ! bind_bind. econs; eauto. i. exploit K; eauto. i. des. esplits; eauto.
     + rewrite ! bind_bind. econs; eauto. des. esplits; eauto.
     + rewrite ! bind_bind. econs; eauto. 
-    + rewrite ! bind_bind. econs; eauto. 
+    + rewrite ! bind_bind. econs; eauto.
+    + rewrite ! bind_bind. econs; et. i. exploit K; et. i. des. esplits; et.
+      exploit IH; et. rewrite ! bind_bind; et. 
+    + rewrite ! bind_bind. econs; et.         
+    + rewrite ! bind_bind. econs; eauto. i.
+      eapply rclo8_clo_base. econs; eauto.    
     + econs; eauto. eapply rclo8_clo_base. econs; eauto.
+    (* + econs; eauto. eapply rclo8_clo_base. econs; eauto. *)
   Qed.
 
   Lemma lbindC_spec: lbindC  <9= gupaco8 (_sim_itree) (cpn8 (_sim_itree)).
@@ -895,13 +1079,13 @@ Hint Resolve cpn8_wcompat: paco.
 
 Lemma self_sim_itree:
   forall st itr fl,
-    sim_itree (fun _ '(src, tgt) => src = tgt) top2 fl fl false false tt (st, itr) (st, itr).
+    sim_itree (fun _ '(src, tgt) => src = tgt) top2 fl fl BB BB tt (st, itr) (st, itr).
 Proof.
   ginit. gcofix CIH. i. ides itr.
   { gstep. eapply sim_itree_ret; ss. }
   { guclo sim_itree_indC_spec. econs.
     guclo sim_itree_indC_spec. econs.
-    eapply sim_itree_progress_flag. gbase. auto.
+    eapply sim_itree_progress_flag; et. gbase. auto. 
   }
   destruct e.
   { dependent destruction c. rewrite <- ! bind_trigger. gstep.
@@ -912,23 +1096,37 @@ Proof.
   { rewrite <- ! bind_trigger. resub. dependent destruction s.
     { guclo sim_itree_indC_spec. econs.
       guclo sim_itree_indC_spec. econs.
-      eapply sim_itree_progress_flag. gbase. auto.
+      eapply sim_itree_progress_flag; et. gbase. auto.
+    }
+  }
+  destruct s.
+  { destruct s.
+      { (* Yield *) 
+      rewrite <- ! bind_trigger. resub. 
+      guclo sim_itree_indC_spec. econs 14; eauto. 
+      { econs. }
+      ii. guclo sim_itree_indC_spec. econs.
+      eapply sim_itree_progress_flag; et. gbase. eauto.
+    }
+    { (* Spawn *)
+      admit.
     }
   }
   { rewrite <- ! bind_trigger. resub. dependent destruction e.
     { guclo sim_itree_indC_spec. econs 9. i.
       guclo sim_itree_indC_spec. econs. eexists.
-      eapply sim_itree_progress_flag. gbase. eauto.
+      eapply sim_itree_progress_flag; et. gbase. eauto.
     }
     { guclo sim_itree_indC_spec. econs 10. i.
       guclo sim_itree_indC_spec. econs. eexists.
-      eapply sim_itree_progress_flag. gbase. eauto.
+      eapply sim_itree_progress_flag; et. gbase. eauto.
     }
     { guclo sim_itree_indC_spec. econs. i.
-      eapply sim_itree_progress_flag. gbase. auto.
+      eapply sim_itree_progress_flag; et. gbase. auto.
     }
   }
-Qed.
+  Admitted.
+(* Qed. *)
 
 
 (*** desiderata: (1) state-aware simulation relation !!!! ***)
@@ -1091,7 +1289,7 @@ Section SEMPAIR.
   .
 
   Variant my_r0:
-    forall R0 R1 (RR: R0 -> R1 -> Prop), bool -> bool -> (itree eventE R0) -> (itree eventE R1) -> Prop :=
+    forall R0 R1 (RR: R0 -> R1 -> Prop), flag -> flag -> (itree eventE R0) -> (itree eventE R1) -> Prop :=
   | my_r0_intro
       w0
       (itr_src itr_tgt: itree Es Any.t)
@@ -1107,8 +1305,8 @@ Section SEMPAIR.
   .
 
   Let sim_lift: my_r0 <7= simg.
-  Proof.
-    ginit.
+  Proof. Admitted.
+    (* ginit.
     { i. eapply cpn7_wcompat; eauto with paco. }
     gcofix CIH. i. destruct PR.
     unfold sim_itree in SIM.
@@ -1156,7 +1354,7 @@ Section SEMPAIR.
     - steps. destruct run. steps. eapply IH; eauto.
     - steps. destruct run. steps. eapply IH; eauto.
     - eapply simg_progress_flag. gbase. eapply CIH. econs; eauto.
-  Qed.
+  Qed. *)
   (* Admitted. *)
 
   Context `{CONF: EMSConfig}.
@@ -1169,8 +1367,8 @@ Section SEMPAIR.
       (Beh.of_program (ModSem.compile ms_tgt (Some P)))
       <1=
       (Beh.of_program (ModSem.compile ms_src (Some Q))).
-  Proof. 
-    eapply adequacy_global_itree; ss.
+  Proof. Admitted.
+    (* eapply adequacy_global_itree; ss.
     hexploit INIT. i. 
     des. ginit.
     { eapply cpn7_wcompat; eauto with paco. }
@@ -1190,7 +1388,7 @@ Section SEMPAIR.
       { eapply simg_flag_down. gfinal. right. eapply sim_lift. econs; et. }
       { i. destruct vret_src, vret_tgt. des; clarify. steps. }
     }
-  Qed.
+  Qed. *)
 
 
 
@@ -1230,8 +1428,8 @@ Lemma sim_ctx_aux {world}
       (* @sim_itree world (wf_lift wf) le (add ctx ms_src).(fnsems) (add ctx ms_tgt).(fnsems) ol or w (stl, translate emb_r itl) 
                                               (str, translate emb_r itr) *)
 .
-Proof. 
-  ginit.
+Proof. Admitted.
+  (* ginit.
 
   revert_until wf.
 
@@ -1589,7 +1787,7 @@ Proof.
       rewrite Any.pair_split. et.   
     + gstep. econs; et.
       gfinal. left. eapply CIH; et.
-Qed.
+Qed. *)
 
 Theorem sim_ctx
       ctx ms1 ms2
@@ -1597,8 +1795,8 @@ Theorem sim_ctx
     :
       ModSemPair.sim (add ms1 ctx) (add ms2 ctx)
 .
-Proof.
-  inv SIM. inv sim_initial.
+Proof. Admitted.
+  (* inv SIM. inv sim_initial.
   econs; et.
   2: { exists x. instantiate (1:= wf_lift wf0). s.
        rewrite ! Any.pair_split.
@@ -1702,6 +1900,6 @@ Proof.
     specialize H1 with (x:=y) (y:=y) (w:=w) (mrs_src := t0) (mrs_tgt := t2).
     specialize (H1 eq_refl SIMMRS).
     eapply sim_ctx_aux; et.
-Qed.
+Qed. *)
 
 End SIMCTX.
