examples/fai/FAI0.v
@@ -1,0 +1,42 @@
+Require Import Coqlib.
+Require Import ITreelib.
+Require Import ImpPrelude.
+Require Import STS.
+Require Import Behavior.
+Require Import ModSem.
+Require Import Skeleton.
+Require Import PCM.
+
+Set Implicit Arguments.
+
+
+
+Section PROOF.
+
+  Definition FAIF: Any.t -> itree Es Any.t :=
+    fun varg =>
+      varg <- varg↓?;;
+      trigger Yield;;;
+      (if negb (val_dec varg (Vint 0))
+      then
+        trigger Yield;;;
+        trigger (Call "fai" [varg]↑);;;
+        trigger Yield
+      else Ret ());;;
+      r <- trigger Yield;;
+      Ret r↑
+    .
+
+  Definition FAISem: ModSem.t := {|
+    ModSem.fnsems := [("FAI", FAIF)];
+    ModSem.init_st := tt↑;
+  |}
+  .
+
+  Definition FAI: Mod.t := {|
+    Mod.get_modsem := fun _ => FAISem;
+    Mod.sk := Sk.unit;
+  |}
+  .
+
+End PROOF.
