examples/fai/FAI1.v
@@ -1,0 +1,48 @@
+Require Import ITreelib.
+Require Import ImpPrelude.
+Require Import STS.
+Require Import Behavior.
+Require Import ModSem.
+Require Import Skeleton.
+Require Import PCM.
+Require Import HoareDef STB.
+Require Import ProofMode.
+Require Import Mem1.
+
+Set Implicit Arguments.
+
+
+
+Section PROOF.
+
+  Context {Σ : GRA.t}.
+  Context `{@GRA.inG memRA Σ}.
+
+  Definition has_n varg n : iProp := (∃ b ofs, ⌜varg = Vptr b ofs⌝ ** OwnM((b, ofs) |-> [Vint n]))%I.
+
+  Definition FAIF: Any.t -> itree Es Any.t :=
+    fun varg =>
+      `varg : val <- varg↓?;;
+      trigger Yield;;;
+      σ <- trigger (Take Σ);;
+      n <- trigger (Take Z);;
+      assume (has_n varg n σ);;;
+      trigger (Call "fai" [varg]↑);;;
+      guarantee (has_n varg (n + 1) σ);;;
+      r <- trigger Yield;;
+      Ret r↑
+    .
+
+  Definition FAISem: ModSem.t := {|
+    ModSem.fnsems := [("FAI", FAIF)];
+    ModSem.init_st := tt↑;
+  |}
+  .
+
+  Definition FAI: Mod.t := {|
+    Mod.get_modsem := fun _ => FAISem;
+    Mod.sk := Sk.unit;
+  |}
+  .
+
+End PROOF.
