examples/fai/Main0.v
@@ -1,0 +1,43 @@
+Require Import Coqlib.
+Require Import ITreelib.
+Require Import ImpPrelude.
+Require Import STS.
+Require Import Behavior.
+Require Import ModSem.
+Require Import Skeleton.
+Require Import PCM.
+
+Set Implicit Arguments.
+
+
+
+Section PROOF.
+
+  Definition mainF: Any.t -> itree Es Any.t :=
+    fun _ =>
+      trigger Yield;;;
+      v <- ccallU "alloc" [Vint 1];;
+      `_ : val <- ccallU "store" [v; Vint 1];;
+      trigger Yield;;;
+      `_ : val <- ccallU "fai" [v];;
+      trigger Yield;;;
+      vint <- ccallU "load" [v];;
+      z <- (pargs [Tint] [vint])?;;
+      trigger (Syscall "print_num" [z]↑ top1);;;
+      r <- trigger Yield;;
+      Ret r↑
+    .
+
+  Definition MainSem: ModSem.t := {|
+    ModSem.fnsems := [("main", mainF)];
+    ModSem.init_st := tt↑;
+  |}
+  .
+
+  Definition Main: Mod.t := {|
+    Mod.get_modsem := fun _ => MainSem;
+    Mod.sk := Sk.unit;
+  |}
+  .
+
+End PROOF.
