examples/fai/Main01proof.v
@@ -1,0 +1,45 @@
+Require Import HoareDef Main0 Main1 Mem1.
+Require Import Coqlib.
+Require Import ImpPrelude.
+Require Import Skeleton.
+Require Import PCM.
+Require Import ModSem Behavior SimModSem SimModSemFacts.
+Require Import Relation_Definitions.
+
+(*** TODO: export these in Coqlib or Universe ***)
+Require Import Relation_Operators.
+Require Import RelationPairs.
+From ITree Require Import
+     Events.MapDefault.
+From ExtLib Require Import
+     Core.RelDec
+     Structures.Maps
+     Data.Map.FMapAList.
+
+Require Import HTactics ProofMode.
+
+Set Implicit Arguments.
+
+Local Open Scope nat_scope.
+
+
+
+Section SIMMODSEM.
+
+  Context `{Σ: GRA.t}.
+  Context `{@GRA.inG memRA Σ}.
+
+  Let W : Type := Any.t * Any.t.
+
+  Let wf: unit -> W -> Prop := fun _ _ => True.
+
+  Theorem correct: refines2 [Main0.Main] [Main1.Main].
+  Proof.
+    eapply adequacy_local2. econs; ss.
+    i. econstructor 1 with (wf:=wf) (le:=top2); et.
+    { ss. }
+    2: { exists tt. ss. }
+    econs; ss. init.
+  Admitted.
+
+End SIMMODSEM.
