spc/Hoareproof0.v
@@ -395,7 +395,7 @@ Section CANCEL.
     forall RT
            mr0 frs 
            ctx0
-           st_src0 st_tgt0 (i0: itree (hCallE +' sE +' eventE) RT)
+           st_src0 st_tgt0 (i0: itree (hCallE +' sE +' schE +' eventE) RT)
            cur
            (ZIP: st_tgt0 = zip_state st_src0 mr0)
            (CTX: ctx0 = frs)
@@ -406,13 +406,13 @@ Section CANCEL.
                 (<<ZIP: st_tgt1 = zip_state st_src1 mrs1>>) /\
                 (<<RET: (v_tgt: Σ * RT) = (frs, v_src)>>))
                 (* (<<RET: (v_tgt: Σ * RT) = (frs ⋅ mrs1, v_src)>>)) *)
-           false false
+           BB BB
            (interp_Es (ModSem.prog ms_mid) (interp_hCallE_mid (stb sk) cur i0) st_src0)
            (interp_Es (ModSem.prog ms_tgt) (interp_hCallE_tgt (stb sk) cur i0 ctx0) st_tgt0)
   .
   Proof.
-  (* Admitted. *)
-    Opaque subevent.
+  Admitted.
+    (* Opaque subevent.
     ginit.
     { i. eapply cpn7_wcompat; eauto with paco. }
     gcofix CIH. i; subst.
@@ -527,7 +527,7 @@ Section CANCEL.
     }
   Unshelve.
     all: try (by exact 0).
-  Qed.
+  Qed. *)
 
   Opaque interp_Es.
 
@@ -548,8 +548,8 @@ Section CANCEL.
                    ret_src = ret_tgt>>)):
     Beh.of_program (@Mod.compile _ CONFT md_tgt) <1=
     Beh.of_program (@Mod.compile _ midConf md_mid).
-  Proof.
-    eapply adequacy_global_itree; ss.
+  Proof. Admitted.
+    (* eapply adequacy_global_itree; ss.
     ginit.
     { eapply cpn7_wcompat; eauto with paco. }
     unfold ModSem.initial_itr, ModSem.initial_itr. Local Opaque ModSem.prog. ss.
@@ -608,6 +608,6 @@ Section CANCEL.
       instantiate (1:=(c1 ⋅ ε ⋅ c)).
       r_wf x0. }
     Unshelve. all: try (exact 0).
-  Qed.
+  Qed. *)
 
 End CANCEL.
